@prefix : <http://www.semanticweb.org/owl/owlapi/turtle#> .
@prefix dc: <http://purl.org/dc/elements/1.1/> .
@prefix chc: <http://www.sirma.com/ontologies/2016/02/culturalHeritageConservation#> .
@prefix emf: <http://ittruse.ittbg.com/ontology/enterpriseManagementFramework#> .
@prefix nga: <http://www.sirma.com/ontologies/2016/02/culturalHeritageConservation/NGA#> .
@prefix owl: <http://www.w3.org/2002/07/owl#> .
@prefix rdf: <http://www.w3.org/1999/02/22-rdf-syntax-ns#> .
@prefix sec: <http://www.sirma.com/ontologies/2014/11/security#> .
@prefix xml: <http://www.w3.org/XML/1998/namespace> .
@prefix xsd: <http://www.w3.org/2001/XMLSchema#> .
@prefix ptop: <http://www.ontotext.com/proton/protontop#> .
@prefix rdfs: <http://www.w3.org/2000/01/rdf-schema#> .
@prefix skos: <http://www.w3.org/2004/02/skos/core#> .
@prefix dcterms: <http://purl.org/dc/terms/> .
@base <http://www.sirma.com/ontologies/2016/02/culturalHeritageConservation/NGA> .

<http://www.sirma.com/ontologies/2016/02/culturalHeritageConservation/NGA> rdf:type owl:Ontology ;
                                                                            owl:imports <http://www.sirma.com/ontologies/2016/02/culturalHeritageConservation> ;
                                                                            dc:subject "Extension of Cultural Heritage Conservation Ontology Model for NGA"@en ;
                                                                            owl:versionInfo "0.1"@en ;
                                                                            dc:creator "Lidiya Dimitrova"@en ;
                                                                            rdfs:label "Extension of Cultural Heritage Conservation Ontology Model for NGA"@en ;
                                                                            dc:rights "What rights?"@en ;
                                                                            rdfs:comment "NGA Extension of Cultural Heritage Conservation Ontology Model for Conservation Space project"@en .

#################################################################
#    Object Properties
#################################################################

###  http://www.sirma.com/ontologies/2016/02/culturalHeritageConservation/NGA#associatedWith
nga:associatedWith rdf:type owl:ObjectProperty ,
                            owl:SymmetricProperty ;
                   rdfs:domain chc:CulturalObject ;
                   rdfs:range chc:CulturalObject ;
                   emf:auditEvent "+addAssociatedWith|-removeAssociatedWith|changeAssociatedWith" ;
                   emf:isSearchable "true"^^xsd:boolean ;
                   dc:creator "Lidiya Dimitrova" ;
                   rdfs:label "is associated with"@en ;
                   skos:definition "Indicates the cultural object is associated with anathor cultural object."@en .


#################################################################
#    Data properties
#################################################################

###  http://www.sirma.com/ontologies/2016/02/culturalHeritageConservation#condition
chc:condition rdf:type owl:DatatypeProperty .


###  http://www.sirma.com/ontologies/2016/02/culturalHeritageConservation/NGA#accessionNumber
nga:accessionNumber rdf:type owl:DatatypeProperty ;
                    rdfs:domain chc:CulturalObject ;
                    rdfs:range xsd:string ;
                    dc:creator "Kiril Penev"@en ;
                    rdfs:comment "" ;
                    rdfs:label "Accession Number"@en ;
                    skos:definition "Unique institutional ID. Can be coded to be human readable and to express, for example, year/lot/number if acquisition or shelf location."@en .


###  http://www.sirma.com/ontologies/2016/02/culturalHeritageConservation/NGA#activityPhase
nga:activityPhase rdf:type owl:DatatypeProperty ;
                  rdfs:range xsd:string ;
                  dc:creator "Lidiya Dimitrova"@en ;
                  rdfs:label "Examination/Treatment Phase"@en ;
                  skos:definition "The stage of the treatment/examination."@en .


###  http://www.sirma.com/ontologies/2016/02/culturalHeritageConservation/NGA#analysisDate
nga:analysisDate rdf:type owl:DatatypeProperty ;
                 rdfs:range xsd:dateTime ;
                 dc:creator "Lidiya Dimitrova" ;
                 rdfs:label "Date of analysis"@en ;
                 skos:definition "The date of any analysis made on the sample."@en .


###  http://www.sirma.com/ontologies/2016/02/culturalHeritageConservation/NGA#analysisSummary
nga:analysisSummary rdf:type owl:DatatypeProperty ;
                    rdfs:range xsd:string ;
                    dc:creator "Lidiya Dimitrova"@en ;
                    rdfs:label "Analysis Summary"@en ;
                    skos:definition "Summary description of the what was found by the analysis on the sample."@en .


###  http://www.sirma.com/ontologies/2016/02/culturalHeritageConservation/NGA#appliedMediaCondition
nga:appliedMediaCondition rdf:type owl:DatatypeProperty ;
                          rdfs:subPropertyOf chc:condition ;
                          rdfs:range xsd:string ;
                          dc:creator "Lidiya Dimitrova"@en ;
                          rdfs:label "Applied Media Condition"@en ;
                          skos:definition "Condition of the media applied to a photograph."@en .


###  http://www.sirma.com/ontologies/2016/02/culturalHeritageConservation/NGA#appliedMediaDescription
nga:appliedMediaDescription rdf:type owl:DatatypeProperty ;
                            rdfs:domain nga:Photograph ;
                            rdfs:range xsd:string ;
                            dc:creator "Lidiya Dimitrova"@en ;
                            rdfs:label "Applied Media Description"@en ;
                            skos:definition "Description of media applied to photograph or to surface coating (eg retouching or hand coloring)"@en .


###  http://www.sirma.com/ontologies/2016/02/culturalHeritageConservation/NGA#artistInstructions
nga:artistInstructions rdf:type owl:DatatypeProperty ;
                       rdfs:domain nga:MediaArt ;
                       rdfs:range xsd:string ;
                       dc:creator "Lidiya Dimitrova"@en ;
                       rdfs:label "Artist Instructions"@en ;
                       skos:definition "Artists description of how the work is to be displayed/installed."@en .


###  http://www.sirma.com/ontologies/2016/02/culturalHeritageConservation/NGA#artistNames
nga:artistNames rdf:type owl:DatatypeProperty ;
                rdfs:domain chc:CulturalObject ;
                rdfs:range xsd:string ;
                dc:creator "Lidiya Dimitrova"@en ;
                rdfs:label "Artist(s)"@en ;
                skos:definition "An entity primarily responsible for creating an object."@en .


###  http://www.sirma.com/ontologies/2016/02/culturalHeritageConservation/NGA#assetCreator
nga:assetCreator rdf:type owl:DatatypeProperty ;
                 rdfs:range xsd:string ;
                 dc:creator "Lidiya Dimitrova"@en ;
                 rdfs:label "Creator"@en ;
                 skos:definition "Name of asset creator  (scanned images or derivative files not created by original photographer)."@en .


###  http://www.sirma.com/ontologies/2016/02/culturalHeritageConservation/NGA#associatedMaterials
nga:associatedMaterials rdf:type owl:DatatypeProperty ;
                        rdfs:domain nga:MediaArt ;
                        rdfs:range xsd:string ;
                        dc:creator "Lidiya Dimitrova"@en ;
                        rdfs:label "Associated Materials"@en ;
                        skos:definition "This would include materials provided by the artist that are used for installation/adjustment/repair of the work of art, but are not actually part of the work of art."@en .


###  http://www.sirma.com/ontologies/2016/02/culturalHeritageConservation/NGA#barCode
nga:barCode rdf:type owl:DatatypeProperty ;
            rdfs:domain nga:Frame ;
            rdfs:range xsd:string ;
            dc:creator "Lidiya Dimitrova"@en ;
            rdfs:label "Bar Code"@en ;
            skos:definition "Symbol representation of the barcode."@en .


###  http://www.sirma.com/ontologies/2016/02/culturalHeritageConservation/NGA#baseCondition
nga:baseCondition rdf:type owl:DatatypeProperty ;
                  rdfs:subPropertyOf chc:condition ;
                  rdfs:range xsd:string ;
                  dc:creator "Lidiya Dimitrova"@en ;
                  rdfs:label "Base Condition"@en ;
                  skos:definition "Description of the condition of the base of the cultural object."@en .


###  http://www.sirma.com/ontologies/2016/02/culturalHeritageConservation/NGA#baseDescription
nga:baseDescription rdf:type owl:DatatypeProperty ;
                    rdfs:domain chc:CulturalObject ;
                    rdfs:range xsd:string ;
                    dc:creator "Lidiya Dimitrova"@en ;
                    rdfs:label "Base Description"@en ;
                    skos:definition "Description of the base for the cultural object, normally on a statue or sculpture. The bottom support of anything; that on which a thing stands or rests."@en .


###  http://www.sirma.com/ontologies/2016/02/culturalHeritageConservation/NGA#bibliography
nga:bibliography rdf:type owl:DatatypeProperty ;
                 rdfs:domain chc:CulturalObject ;
                 rdfs:range xsd:string ;
                 dc:creator "Lidiya Dimitrova"@en ;
                 rdfs:label "Bibliography"@en ;
                 skos:definition """A bibliography is a list of all of the sources used (whether referenced or not) in the process of researching. In general, a bibliography should include:
    · the authors' names
    · the titles of the works
    · the names and locations of the companies that published your copies of the sources
    · the dates your copies were published
    · the page numbers of your sources (if they are part of multi-source volumes)"""@en .


###  http://www.sirma.com/ontologies/2016/02/culturalHeritageConservation/NGA#binderCondition
nga:binderCondition rdf:type owl:DatatypeProperty ;
                    rdfs:subPropertyOf chc:condition ;
                    rdfs:range xsd:string ;
                    dc:creator "Lidiya Dimitrova"@en ;
                    rdfs:label "Binder Condition"@en ;
                    skos:definition "Description of the condition of the binder."@en .


###  http://www.sirma.com/ontologies/2016/02/culturalHeritageConservation/NGA#binderMaterial
nga:binderMaterial rdf:type owl:DatatypeProperty ;
                   rdfs:domain nga:Photograph ;
                   rdfs:range xsd:string ;
                   dc:creator "Lidiya Dimitrova" ;
                   rdfs:label "Binder Material"@en ;
                   skos:definition "Description of any material that holds the light sensitive materials."@en .


###  http://www.sirma.com/ontologies/2016/02/culturalHeritageConservation/NGA#bindingCovering
nga:bindingCovering rdf:type owl:DatatypeProperty ;
                    rdfs:domain nga:BoundVolume ;
                    rdfs:range xsd:string ;
                    dc:creator "Lidiya Dimitrova" ;
                    rdfs:label "Covering, decoration/finishing"@en ;
                    skos:definition "Description of stamping, labels, or decoration to the binding."@en .


###  http://www.sirma.com/ontologies/2016/02/culturalHeritageConservation/NGA#bindingStyle
nga:bindingStyle rdf:type owl:DatatypeProperty ;
                 rdfs:domain nga:BoundVolume ;
                 rdfs:range xsd:string ;
                 dc:creator "Lidiya Dimitrova" ;
                 rdfs:label "Binding Style"@en ;
                 skos:definition "Description of the binding style, materials and construction."@en .


###  http://www.sirma.com/ontologies/2016/02/culturalHeritageConservation/NGA#borrowerName
nga:borrowerName rdf:type owl:DatatypeProperty ;
                 rdfs:range xsd:string ;
                 dc:creator "Lidiya Dimitrova" ;
                 rdfs:label "Borrower"@en ;
                 skos:definition "The Institution that has borrowed the Cultural Object (outgoing Loan)"@en .


###  http://www.sirma.com/ontologies/2016/02/culturalHeritageConservation/NGA#callNumber
nga:callNumber rdf:type owl:DatatypeProperty ;
               rdfs:domain chc:CulturalObject ;
               rdfs:range xsd:string ;
               dc:creator "Lidiya Dimitrova"@en ;
               rdfs:label "Call Number"@en ;
               skos:definition "NGA Library number"@en .


###  http://www.sirma.com/ontologies/2016/02/culturalHeritageConservation/NGA#captureDevice
nga:captureDevice rdf:type owl:DatatypeProperty ;
                  rdfs:range xsd:string ;
                  dc:creator "Lidiya Dimitrova"@en ;
                  rdfs:label "Creator"@en ;
                  skos:definition "The name of the camera or scanner."@en .


###  http://www.sirma.com/ontologies/2016/02/culturalHeritageConservation/NGA#caseCondition
nga:caseCondition rdf:type owl:DatatypeProperty ;
                  rdfs:subPropertyOf chc:condition ;
                  rdfs:range xsd:string ;
                  dc:creator "Lidiya Dimitrova"@en ;
                  rdfs:label "Case Condition"@en ;
                  skos:definition "Description of the case condition."@en .


###  http://www.sirma.com/ontologies/2016/02/culturalHeritageConservation/NGA#caseDescription
nga:caseDescription rdf:type owl:DatatypeProperty ;
                    rdfs:domain nga:Photograph ;
                    rdfs:range xsd:string ;
                    dc:creator "Lidiya Dimitrova"@en ;
                    rdfs:label "Case Description"@en ;
                    skos:definition "Description of case, including exterior, hinge, interior, and textile if applicable."@en .


###  http://www.sirma.com/ontologies/2016/02/culturalHeritageConservation/NGA#catalogueRaisonneRef
nga:catalogueRaisonneRef rdf:type owl:DatatypeProperty ;
                         rdfs:domain chc:CulturalObject ;
                         rdfs:range xsd:string ;
                         dc:creator "Lidiya Dimitrova"@en ;
                         rdfs:label "Catalogue Raisonne Number"@en ;
                         skos:definition "A global number of  the art work that appears in Catalogue Raisonne."@en .


###  http://www.sirma.com/ontologies/2016/02/culturalHeritageConservation/NGA#century
nga:century rdf:type owl:DatatypeProperty ;
            rdfs:domain nga:Frame ;
            rdfs:range xsd:string ;
            dc:creator "Lidiya Dimitrova" ;
            rdfs:label "Century"@en ;
            skos:definition "The art object century."@en .


###  http://www.sirma.com/ontologies/2016/02/culturalHeritageConservation/NGA#collation
nga:collation rdf:type owl:DatatypeProperty ;
              rdfs:domain nga:BoundVolume ;
              rdfs:range xsd:string ;
              dc:creator "Lidiya DImitrova"@en ;
              rdfs:label "Textblock, collation"@en ;
              skos:definition "Description of the printer's imposition and organization of the gatherings in a textblock, expressed in a shorthand formula"@en .


###  http://www.sirma.com/ontologies/2016/02/culturalHeritageConservation/NGA#collection
nga:collection rdf:type owl:DatatypeProperty ;
               rdfs:domain chc:CulturalObject ;
               rdfs:range xsd:string ;
               dc:creator "Lidiya Dimitrova"@en ;
               rdfs:label "Collection"@en ;
               skos:definition "NGA library grouping."@en .


###  http://www.sirma.com/ontologies/2016/02/culturalHeritageConservation/NGA#contactDate
nga:contactDate rdf:type owl:DatatypeProperty ;
                rdfs:range xsd:dateTime ;
                dc:creator "Lidiya Dimitrova"@en ;
                rdfs:label "Date of Contact"@en ;
                skos:definition "Date of Contact."@en .


###  http://www.sirma.com/ontologies/2016/02/culturalHeritageConservation/NGA#contactPerson
nga:contactPerson rdf:type owl:DatatypeProperty ;
                  rdfs:range xsd:string ;
                  dc:creator "Lidiya Dimitrova"@en ;
                  rdfs:label "Contact Person"@en ;
                  skos:definition "Contact Person"@en .


###  http://www.sirma.com/ontologies/2016/02/culturalHeritageConservation/NGA#countryName
nga:countryName rdf:type owl:DatatypeProperty ;
                rdfs:domain nga:Frame ;
                rdfs:range xsd:string ;
                dc:creator "Lidiya Dimitrova" ;
                rdfs:label "Country/Region"@en ;
                skos:definition "The country/region to which the art object is related."@en .


###  http://www.sirma.com/ontologies/2016/02/culturalHeritageConservation/NGA#creationDates
nga:creationDates rdf:type owl:DatatypeProperty ;
                  rdfs:domain chc:CulturalObject ;
                  rdfs:range xsd:string ;
                  dc:creator "Lidiya Dimitrova" ;
                  rdfs:label "Create Date(s)"@en ;
                  skos:definition "Start/end dates and qualifiers such as \"circa\", \"before\", etc. Can have historical records of former attributions of creation dates."@en .


###  http://www.sirma.com/ontologies/2016/02/culturalHeritageConservation/NGA#creditLine
nga:creditLine rdf:type owl:DatatypeProperty ;
               rdfs:domain chc:CulturalObject ;
               rdfs:range xsd:string ;
               dc:creator "Lidiya Dimitrova" ;
               rdfs:label "Credit Line/Collection"@en ;
               skos:definition "Public credit line for the object. "@en .


###  http://www.sirma.com/ontologies/2016/02/culturalHeritageConservation/NGA#culturalObjectViewDescription
nga:culturalObjectViewDescription rdf:type owl:DatatypeProperty ;
                                  rdfs:range xsd:string ;
                                  dc:creator "Lidiya Dimitrova"@en ;
                                  rdfs:label "View Description"@en ;
                                  skos:definition "The view of the cultural object."@en .


###  http://www.sirma.com/ontologies/2016/02/culturalHeritageConservation/NGA#curatorialRemarks
nga:curatorialRemarks rdf:type owl:DatatypeProperty ;
                      rdfs:domain chc:CulturalObject ;
                      rdfs:range xsd:string ;
                      dc:creator "Lidiya Dimitrova" ;
                      rdfs:label "Curatorial Remarks"@en ;
                      skos:definition "Notes made by the curator."@en .


###  http://www.sirma.com/ontologies/2016/02/culturalHeritageConservation/NGA#currentLocation
nga:currentLocation rdf:type owl:DatatypeProperty ;
                    rdfs:domain chc:CulturalObject ;
                    rdfs:range xsd:string ;
                    dc:creator "Lidiya Dimitrova" ;
                    rdfs:label "Current Location"@en ;
                    skos:definition "The location that the object is physically resides currently."@en .


###  http://www.sirma.com/ontologies/2016/02/culturalHeritageConservation/NGA#dateCompleted
nga:dateCompleted rdf:type owl:DatatypeProperty ;
                  rdfs:range xsd:dateTime ;
                  emf:isSearchable "true"^^xsd:boolean ;
                  dc:creator "Malvina Makarieva" ;
                  rdfs:label "Date completed"@en ;
                  skos:definition "Defines the date when report was completed. "@en .


###  http://www.sirma.com/ontologies/2016/02/culturalHeritageConservation/NGA#design
nga:design rdf:type owl:DatatypeProperty ;
           rdfs:domain chc:CulturalObject ;
           rdfs:range xsd:string ;
           dc:creator "Lidiya Dimitrova"@en ;
           rdfs:label "Design"@en ;
           skos:definition "Description of the art object design. The arrangement of the features as produced from following a plan."@en .


###  http://www.sirma.com/ontologies/2016/02/culturalHeritageConservation/NGA#designatedOpening
nga:designatedOpening rdf:type owl:DatatypeProperty ;
                      rdfs:range xsd:string ;
                      dc:creator "Lidiya Dimitrova"@en ;
                      rdfs:label "Designated Opening"@en ;
                      skos:definition "The page to be displayed on the exhibition."@en .


###  http://www.sirma.com/ontologies/2016/02/culturalHeritageConservation/NGA#designatedOpeningCondition
nga:designatedOpeningCondition rdf:type owl:DatatypeProperty ;
                               rdfs:subPropertyOf chc:condition ;
                               rdfs:range xsd:string ;
                               dc:creator "Lidiya Dimitrova"@en ;
                               rdfs:label "Designated Opening Condition"@en ;
                               skos:definition "Description of the case designated opening condition."@en .


###  http://www.sirma.com/ontologies/2016/02/culturalHeritageConservation/NGA#displayedPages
nga:displayedPages rdf:type owl:DatatypeProperty ;
                   rdfs:range xsd:string ;
                   dc:creator "Lidiya Dimitrova"@en ;
                   rdfs:label "Displayed Pages"@en ;
                   skos:definition "Identification of pages from Bound Volume that will be displayed in case the page does not have accession by itself."@en .


###  http://www.sirma.com/ontologies/2016/02/culturalHeritageConservation/NGA#distinguishingMarks
nga:distinguishingMarks rdf:type owl:DatatypeProperty ;
                        rdfs:domain chc:CulturalObject ;
                        rdfs:range xsd:string ;
                        dc:creator "Lidiya Dimitrova"@en ;
                        rdfs:label "Distinguishing Marks"@en ;
                        skos:definition "Indication of distinguishing marks that have been applied to an object, including manufacturer's marks and labels, publisher's and printer's blind stamps."@en .


###  http://www.sirma.com/ontologies/2016/02/culturalHeritageConservation/NGA#donorName
nga:donorName rdf:type owl:DatatypeProperty ;
              rdfs:domain nga:Frame ;
              rdfs:range xsd:string ;
              dc:creator "Lidiya Dimitrova"@en ;
              rdfs:label "Donor Name"@en ;
              skos:definition "Name of the donor of the frame."@en .


###  http://www.sirma.com/ontologies/2016/02/culturalHeritageConservation/NGA#edition
nga:edition rdf:type owl:DatatypeProperty ;
            rdfs:domain chc:CulturalObject ;
            rdfs:range xsd:string ;
            dc:creator "Lidiya Dimitrova" ;
            rdfs:label "Edition"@en ;
            skos:definition "Number of the volumn or set, usually includes year."@en .


###  http://www.sirma.com/ontologies/2016/02/culturalHeritageConservation/NGA#environmentalRequirements
nga:environmentalRequirements rdf:type owl:DatatypeProperty ;
                              rdfs:domain chc:CulturalObject ;
                              rdfs:range xsd:string ;
                              dc:creator "Lidiya Dimitrova"@en ;
                              rdfs:label "Environmental Notes"@en ;
                              skos:definition "Description of any special environmental notes that the cultural object may require."@en .


###  http://www.sirma.com/ontologies/2016/02/culturalHeritageConservation/NGA#essentialComponents
nga:essentialComponents rdf:type owl:DatatypeProperty ;
                        rdfs:domain chc:CulturalObject ;
                        rdfs:range xsd:string ;
                        dc:creator "Lidiya Dimitrova"@en ;
                        rdfs:label "Essential Components"@en ;
                        skos:definition "The parts of the artwork that artist indicates cannot be changed or replaced"@en .


###  http://www.sirma.com/ontologies/2016/02/culturalHeritageConservation/NGA#estimatedExpenses
nga:estimatedExpenses rdf:type owl:DatatypeProperty ;
                      rdfs:range xsd:string ;
                      dc:creator "Lidiya Dimitrova"@en ;
                      rdfs:label "Estimated Expenses"@en ;
                      skos:definition "Estimated expenses for the project"@en .


###  http://www.sirma.com/ontologies/2016/02/culturalHeritageConservation/NGA#exhibitionDescription
nga:exhibitionDescription rdf:type owl:DatatypeProperty ;
                          rdfs:range xsd:string ;
                          dc:creator "Malvina Makarieva"@en ;
                          rdfs:label "Exhibition"@en ;
                          skos:definition "Name of the exhibition associated with the object."@en .


###  http://www.sirma.com/ontologies/2016/02/culturalHeritageConservation/NGA#exhibitionId
nga:exhibitionId rdf:type owl:DatatypeProperty ;
                 rdfs:range xsd:string ;
                 dc:creator "Lidiya Dimitrova"@en ;
                 rdfs:label "Exhibition ID"@en ;
                 skos:definition "The tracking number to track each object with in an Incoming or outgoing Loans for an Exhibition."@en .


###  http://www.sirma.com/ontologies/2016/02/culturalHeritageConservation/NGA#expectedOutcome
nga:expectedOutcome rdf:type owl:DatatypeProperty ;
                    rdfs:range xsd:string ;
                    dc:creator "Lidiya Dimitrova"@en ;
                    rdfs:label "Expected Outcome"@en ;
                    skos:definition "Expected outcome of a project"@en .


###  http://www.sirma.com/ontologies/2016/02/culturalHeritageConservation/NGA#fabricationMethod
nga:fabricationMethod rdf:type owl:DatatypeProperty ;
                      rdfs:domain chc:CulturalObject ;
                      rdfs:range xsd:string ;
                      dc:creator "Lidiya Dimitrova"@en ;
                      rdfs:label "Fabrication Description"@en ;
                      skos:definition "Description of the fabrication method of the art object."@en .


###  http://www.sirma.com/ontologies/2016/02/culturalHeritageConservation/NGA#frameCondition
nga:frameCondition rdf:type owl:DatatypeProperty ;
                   rdfs:subPropertyOf chc:condition ;
                   rdfs:range xsd:string ;
                   dc:creator "Lidiya Dimitrova"@en ;
                   rdfs:label "Frame Conditionn"@en ;
                   skos:definition "Description of condition of the frame."@en .


###  http://www.sirma.com/ontologies/2016/02/culturalHeritageConservation/NGA#frameDescription
nga:frameDescription rdf:type owl:DatatypeProperty ;
                     rdfs:domain chc:CulturalObject ;
                     rdfs:range xsd:string ;
                     dc:creator "Lidiya Dimitrova"@en ;
                     rdfs:label "Frame Description"@en ;
                     skos:definition "Description of the framing overall process and material, the frame itself, if part of the original art object or if the object is permanently framed in storage. Include glazing, framing package and backing."@en .


###  http://www.sirma.com/ontologies/2016/02/culturalHeritageConservation/NGA#frameInnerDimensions
nga:frameInnerDimensions rdf:type owl:DatatypeProperty ;
                         rdfs:domain nga:Frame ;
                         rdfs:range xsd:string ;
                         dc:creator "Lidiya Dimitrova"@en ;
                         rdfs:label "Inner Dimensions"@en ;
                         skos:definition "Inside dimension of the Frame (height and width)"@en .


###  http://www.sirma.com/ontologies/2016/02/culturalHeritageConservation/NGA#frameMoldingWidth
nga:frameMoldingWidth rdf:type owl:DatatypeProperty ;
                      rdfs:domain nga:Frame ;
                      rdfs:range xsd:string ;
                      dc:creator "Lidiya Dimitrova"@en ;
                      rdfs:label "Molding"@en ;
                      skos:definition "The measurement from the site edge to the outer edge of the frame."@en .


###  http://www.sirma.com/ontologies/2016/02/culturalHeritageConservation/NGA#frameNotes
nga:frameNotes rdf:type owl:DatatypeProperty ;
               rdfs:domain nga:Frame ;
               rdfs:range xsd:string ;
               dc:creator "Lidiya Dimitrova"@en ;
               rdfs:label "Frame Notes"@en ;
               skos:definition "Additinal notes on the frame condition."@en .


###  http://www.sirma.com/ontologies/2016/02/culturalHeritageConservation/NGA#frameNumber
nga:frameNumber rdf:type owl:DatatypeProperty ;
                rdfs:domain nga:Frame ;
                rdfs:range xsd:string ;
                dc:creator "Lidiya Dimitrova"@en ;
                rdfs:label "Frame Number"@en ;
                skos:definition "Unique institutional Frame ID."@en .


###  http://www.sirma.com/ontologies/2016/02/culturalHeritageConservation/NGA#frameOutsideDimensions
nga:frameOutsideDimensions rdf:type owl:DatatypeProperty ;
                           rdfs:domain nga:Frame ;
                           rdfs:range xsd:string ;
                           dc:creator "Lidiya Dimitrova"@en ;
                           rdfs:label "Outside Dimensions"@en ;
                           skos:definition "Outer dimension of the Frame (height and width)"@en .


###  http://www.sirma.com/ontologies/2016/02/culturalHeritageConservation/NGA#frameQuantity
nga:frameQuantity rdf:type owl:DatatypeProperty ;
                  rdfs:domain nga:Frame ;
                  rdfs:range xsd:string ;
                  dc:creator "Lidiya Dimitrova"@en ;
                  rdfs:label "Quantity"@en ;
                  skos:definition "The count of the same type of the frame that are held in inventory."@en .


###  http://www.sirma.com/ontologies/2016/02/culturalHeritageConservation/NGA#frameRabbetDepth
nga:frameRabbetDepth rdf:type owl:DatatypeProperty ;
                     rdfs:domain nga:Frame ;
                     rdfs:range xsd:string ;
                     dc:creator "Lidiya Dimitrova"@en ;
                     rdfs:label "Rabbet Depth"@en ;
                     skos:definition "Outer dimension of the Frame (height and width)"@en .


###  http://www.sirma.com/ontologies/2016/02/culturalHeritageConservation/NGA#frameShape
nga:frameShape rdf:type owl:DatatypeProperty ;
               rdfs:domain nga:Frame ;
               rdfs:range xsd:string ;
               dc:creator "Lidiya Dimitrova"@en ;
               rdfs:label "Shape"@en ;
               skos:definition "Description of the frame shape."@en .


###  http://www.sirma.com/ontologies/2016/02/culturalHeritageConservation/NGA#frameSiteSize
nga:frameSiteSize rdf:type owl:DatatypeProperty ;
                  rdfs:domain nga:Frame ;
                  rdfs:range xsd:string ;
                  dc:creator "Lidiya Dimitrova"@en ;
                  rdfs:label "Site Size"@en ;
                  skos:definition "The size of the opening from the front of the frame.  "@en .


###  http://www.sirma.com/ontologies/2016/02/culturalHeritageConservation/NGA#framingPackage
nga:framingPackage rdf:type owl:DatatypeProperty ;
                   rdfs:domain chc:CulturalObject ;
                   rdfs:range xsd:string ;
                   dc:creator "Lidiya Dimitrova"@en ;
                   rdfs:label "Framing Package"@en ;
                   skos:definition "Description of framing package components put together by the institution including frame, glazing, and backing"@en .


###  http://www.sirma.com/ontologies/2016/02/culturalHeritageConservation/NGA#framingPackageCondition
nga:framingPackageCondition rdf:type owl:DatatypeProperty ;
                            rdfs:subPropertyOf chc:condition ;
                            rdfs:range xsd:string ;
                            dc:creator "Lidiya Dimitrova"@en ;
                            rdfs:label "Framing Package Condition"@en ;
                            skos:definition "Description of the condition of the cultural object framing package."@en .


###  http://www.sirma.com/ontologies/2016/02/culturalHeritageConservation/NGA#glazeDescription
nga:glazeDescription rdf:type owl:DatatypeProperty ;
                     rdfs:domain chc:CulturalObject ;
                     rdfs:range xsd:string ;
                     dc:creator "Lidiya Dimitrova"@en ;
                     rdfs:label "Glaze"@en ;
                     skos:definition "Technical description of the glazing or any unusual glazing requirement such as Optium for a friable drawing. The glaze is a translucent colored material, usually a varnish, used as a painting technique."@en .


###  http://www.sirma.com/ontologies/2016/02/culturalHeritageConservation/NGA#handlingRequirements
nga:handlingRequirements rdf:type owl:DatatypeProperty ;
                         rdfs:domain chc:CulturalObject ;
                         rdfs:range xsd:string ;
                         dc:creator "Lidiya Dimitrova"@en ;
                         rdfs:label "Humidity Requirements "@en ;
                         skos:definition "Description of any special handling that the cultural object may require."@en .


###  http://www.sirma.com/ontologies/2016/02/culturalHeritageConservation/NGA#homeLocation
nga:homeLocation rdf:type owl:DatatypeProperty ;
                 rdfs:domain chc:CulturalObject ;
                 rdfs:range xsd:string ;
                 dc:creator "Lidiya Dimitrova"@en ;
                 rdfs:label "Home Location"@en ;
                 skos:definition "A gallery, storage location or  place within the organizatio where the cultural object normally is."@en .


###  http://www.sirma.com/ontologies/2016/02/culturalHeritageConservation/NGA#housingCondition
nga:housingCondition rdf:type owl:DatatypeProperty ;
                     rdfs:subPropertyOf chc:condition ;
                     rdfs:range xsd:string ;
                     dc:creator "Lidiya Dimitrova"@en ;
                     rdfs:label "Housing Condition"@en ;
                     skos:definition "Description of the condition of the housing of the cultural object."@en .


###  http://www.sirma.com/ontologies/2016/02/culturalHeritageConservation/NGA#housingDescription
nga:housingDescription rdf:type owl:DatatypeProperty ;
                       rdfs:domain chc:CulturalObject ;
                       rdfs:range xsd:string ;
                       dc:creator "Lidiya Dimitrova"@en ;
                       rdfs:label "Housing Description"@en ;
                       skos:definition "Description of the permanent/important/original housing, such as box, slip case, original mats or folders, its materials and construction."@en .


###  http://www.sirma.com/ontologies/2016/02/culturalHeritageConservation/NGA#imageCapturedSource
nga:imageCapturedSource rdf:type owl:DatatypeProperty ;
                        rdfs:range xsd:string ;
                        dc:creator "Lidiya Dimitrova"@en ;
                        rdfs:label "Captured Source"@en ;
                        skos:definition "The source of the image. Information related to the origination of the image (where it came from)."@en .


###  http://www.sirma.com/ontologies/2016/02/culturalHeritageConservation/NGA#imageLayerCondition
nga:imageLayerCondition rdf:type owl:DatatypeProperty ;
                        rdfs:subPropertyOf chc:condition ;
                        rdfs:range xsd:string ;
                        dc:creator "Lidiya Dimitrova"@en ;
                        rdfs:label "Image Layer Condition"@en ;
                        skos:definition "Description of the condition of the image layer."@en .


###  http://www.sirma.com/ontologies/2016/02/culturalHeritageConservation/NGA#imageLayerDescription
nga:imageLayerDescription rdf:type owl:DatatypeProperty ;
                          rdfs:domain nga:Photograph ;
                          rdfs:range xsd:string ;
                          dc:creator "Lidiya Dimitrova"@en ;
                          rdfs:label "Image Layer Description"@en ;
                          skos:definition "Description of the final image layer of photograph."@en .


###  http://www.sirma.com/ontologies/2016/02/culturalHeritageConservation/NGA#imageOriginalIdentifier
nga:imageOriginalIdentifier rdf:type owl:DatatypeProperty ;
                            rdfs:range xsd:string ;
                            dc:creator "Lidiya Dimitrova"@en ;
                            rdfs:label "Original Identifier"@en ;
                            skos:definition "Name of the file from which a user creates the derivative. .DNG, raw, master ."@en .


###  http://www.sirma.com/ontologies/2016/02/culturalHeritageConservation/NGA#imageProductDate
nga:imageProductDate rdf:type owl:DatatypeProperty ;
                     rdfs:range xsd:dateTime ;
                     dc:creator "Lidiya Dimitrova"@en ;
                     rdfs:label "Product Date"@en ;
                     skos:definition "The date that the image was produced. "@en .


###  http://www.sirma.com/ontologies/2016/02/culturalHeritageConservation/NGA#imageProductType
nga:imageProductType rdf:type owl:DatatypeProperty ;
                     rdfs:range xsd:string ;
                     dc:creator "Lidiya Dimitrova"@en ;
                     rdfs:label "Product Type"@en ;
                     skos:definition "The product type defines if the image is original raw data or product derivative"@en .


###  http://www.sirma.com/ontologies/2016/02/culturalHeritageConservation/NGA#imageSourceInstitution
nga:imageSourceInstitution rdf:type owl:DatatypeProperty ;
                           rdfs:range xsd:string ;
                           dc:creator "Lidiya Dimitrova"@en ;
                           rdfs:label "Source Institution"@en ;
                           skos:definition "TSource-Institution of the image, department."@en .


###  http://www.sirma.com/ontologies/2016/02/culturalHeritageConservation/NGA#imageSourceType
nga:imageSourceType rdf:type owl:DatatypeProperty ;
                    rdfs:range xsd:string ;
                    dc:creator "Lidiya Dimitrova"@en ;
                    rdfs:label "Source Type"@en ;
                    skos:definition "The format of the source image."@en .


###  http://www.sirma.com/ontologies/2016/02/culturalHeritageConservation/NGA#incomingLoanNumber
nga:incomingLoanNumber rdf:type owl:DatatypeProperty ;
                       rdfs:range xsd:string ;
                       dc:creator "Lidiya Dimitrova"@en ;
                       rdfs:label "In Coming Loan Number"@en ;
                       skos:definition "Unique  number that is assigned to a Loan for an Exhibition inside of the organization."@en .


###  http://www.sirma.com/ontologies/2016/02/culturalHeritageConservation/NGA#inscriptions
nga:inscriptions rdf:type owl:DatatypeProperty ;
                 rdfs:domain chc:CulturalObject ;
                 rdfs:range xsd:string ;
                 dc:creator "Lidiya Dimitrova" ;
                 rdfs:label "Inscription(s)"@en ;
                 skos:definition "Description of any writing or printing on the object's obverse or reverse. Artist signature, dealer marks, inventory codes, etc."@en .


###  http://www.sirma.com/ontologies/2016/02/culturalHeritageConservation/NGA#installationRequirements
nga:installationRequirements rdf:type owl:DatatypeProperty ;
                             rdfs:domain chc:CulturalObject ;
                             rdfs:range xsd:string ;
                             dc:creator "Lidiya Dimitrova" ;
                             rdfs:label "Installation Requirements" ;
                             skos:definition "Any special Installation Instruction that the cultural object may require" .


###  http://www.sirma.com/ontologies/2016/02/culturalHeritageConservation/NGA#laminateCondition
nga:laminateCondition rdf:type owl:DatatypeProperty ;
                      rdfs:subPropertyOf chc:condition ;
                      rdfs:range xsd:string ;
                      dc:creator "Lidiya Dimitrova"@en ;
                      rdfs:label "Laminate Condition"@en ;
                      skos:definition "Description of the laminate condition."@en .


###  http://www.sirma.com/ontologies/2016/02/culturalHeritageConservation/NGA#laminateDescription
nga:laminateDescription rdf:type owl:DatatypeProperty ;
                        rdfs:domain nga:Photograph ;
                        rdfs:range xsd:string ;
                        dc:creator "Lidiya Dimitrova"@en ;
                        rdfs:label "Laminate Description"@en ;
                        skos:definition "Description of glazing, face mounting, or laminate (eg face mounted photographs, plastic laminate, ambrotype, integral frame)."@en .


###  http://www.sirma.com/ontologies/2016/02/culturalHeritageConservation/NGA#legacy
nga:legacy rdf:type owl:DatatypeProperty ;
           rdfs:range xsd:string ;
           emf:isSearchable "true"^^xsd:boolean ;
           dc:creator "Malvina Makarieva"@en ;
           rdfs:label "Legacy"@en ;
           skos:definition "Identifies is the document is legacy or not."@en .


###  http://www.sirma.com/ontologies/2016/02/culturalHeritageConservation/NGA#lenderName
nga:lenderName rdf:type owl:DatatypeProperty ;
               rdfs:range xsd:string ;
               dc:creator "Lidiya Dimitrova" ;
               rdfs:label "Lender"@en ;
               skos:definition "The institution that has lend the Cultural Object for the Exhibition."@en .


###  http://www.sirma.com/ontologies/2016/02/culturalHeritageConservation/NGA#lightType
nga:lightType rdf:type owl:DatatypeProperty ;
              rdfs:range xsd:string ;
              dc:creator "Lidiya Dimitrova"@en ;
              rdfs:label "Light Type"@en ;
              skos:definition "The type of light used for the photograph to be taken."@en .


###  http://www.sirma.com/ontologies/2016/02/culturalHeritageConservation/NGA#loanId
nga:loanId rdf:type owl:DatatypeProperty ;
           rdfs:range xsd:string ;
           dc:creator "Malvina Makarieva"@en ;
           rdfs:label "Loan ID"@en ;
           skos:definition "The Loan ID associated with the object; (free text)."@en .


###  http://www.sirma.com/ontologies/2016/02/culturalHeritageConservation/NGA#manipulateType
nga:manipulateType rdf:type owl:DatatypeProperty ;
                   rdfs:range xsd:string ;
                   dc:creator "Lidiya Dimitrova"@en ;
                   rdfs:label "Manipulate Type"@en ;
                   skos:definition "The manipulate type of the image e.g raw, histogram, color."@en .


###  http://www.sirma.com/ontologies/2016/02/culturalHeritageConservation/NGA#manufactureMethod
nga:manufactureMethod rdf:type owl:DatatypeProperty ;
                      rdfs:domain chc:CulturalObject ;
                      rdfs:range xsd:string ;
                      dc:creator "Lidiya Dimitrova"@en ;
                      rdfs:label "Method Of Manufacture"@en ;
                      skos:definition "Specific details of how an object is made based on examination"@en .


###  http://www.sirma.com/ontologies/2016/02/culturalHeritageConservation/NGA#manufacturerName
nga:manufacturerName rdf:type owl:DatatypeProperty ;
                     rdfs:range xsd:string ;
                     dc:creator "Lidiya Dimitrova"@en ;
                     rdfs:label "Manufacturer"@en ;
                     skos:definition "The name of the product manufacturer"@en .


###  http://www.sirma.com/ontologies/2016/02/culturalHeritageConservation/NGA#matAttachmentCondition
nga:matAttachmentCondition rdf:type owl:DatatypeProperty ;
                           rdfs:subPropertyOf chc:condition ;
                           rdfs:range xsd:string ;
                           dc:creator "Lidiya Dimitrova"@en ;
                           rdfs:label "Attachment Condition"@en ;
                           skos:definition "Description of the condition of the cultural object attachment to the mat."@en .


###  http://www.sirma.com/ontologies/2016/02/culturalHeritageConservation/NGA#matAttachmentDescription
nga:matAttachmentDescription rdf:type owl:DatatypeProperty ;
                             rdfs:domain chc:CulturalObject ;
                             rdfs:range xsd:string ;
                             dc:creator "Lidiya Dimitrova"@en ;
                             rdfs:label "Attachment Description"@en ;
                             skos:definition "Description of how  the object is attached to the mat. (attachment method)"@en .


###  http://www.sirma.com/ontologies/2016/02/culturalHeritageConservation/NGA#matCondition
nga:matCondition rdf:type owl:DatatypeProperty ;
                 rdfs:subPropertyOf chc:condition ;
                 rdfs:range xsd:string ;
                 dc:creator "Lidiya Dimitrova"@en ;
                 rdfs:label "Mat Condition"@en ;
                 skos:definition "Description of the mat condition."@en .


###  http://www.sirma.com/ontologies/2016/02/culturalHeritageConservation/NGA#matDescription
nga:matDescription rdf:type owl:DatatypeProperty ;
                   rdfs:domain chc:CulturalObject ;
                   rdfs:range xsd:string ;
                   dc:creator "Lidiya Dimitrova"@en ;
                   rdfs:label "Attachment Description"@en ;
                   skos:definition "Description of how  the object is attached to the mat. (attachment method)"@en .


###  http://www.sirma.com/ontologies/2016/02/culturalHeritageConservation/NGA#materialType
nga:materialType rdf:type owl:DatatypeProperty ;
                 rdfs:range xsd:string ;
                 dc:creator "Lidiya Dimitrova"@en ;
                 rdfs:label "Material type"@en ;
                 skos:definition "Description of the material type."@en .


###  http://www.sirma.com/ontologies/2016/02/culturalHeritageConservation/NGA#mediaCondition
nga:mediaCondition rdf:type owl:DatatypeProperty ;
                   rdfs:subPropertyOf chc:condition ;
                   rdfs:range xsd:string ;
                   dc:creator "Lidiya Dimitrova"@en ;
                   rdfs:label "Media Condition"@en ;
                   skos:definition "Description of the condition of the media  such as media flaking, cracking, loss media abrasion, scratches, burnishing, media fading, media friable."@en .


###  http://www.sirma.com/ontologies/2016/02/culturalHeritageConservation/NGA#mediaDescription
nga:mediaDescription rdf:type owl:DatatypeProperty ;
                     rdfs:domain chc:CulturalObject ;
                     rdfs:range xsd:string ;
                     dc:creator "Lidiya Dimitrova"@en ;
                     rdfs:label "Media"@en ;
                     skos:definition "Description of the media used for the cultural object."@en .


###  http://www.sirma.com/ontologies/2016/02/culturalHeritageConservation/NGA#medium
nga:medium rdf:type owl:DatatypeProperty ;
           rdfs:domain chc:CulturalObject ;
           rdfs:range xsd:string ;
           dc:creator "Lidiya Dimitrova"@en ;
           rdfs:label "Material/Medium (very general)"@en ;
           skos:definition "Medium description often used for public."@en .


###  http://www.sirma.com/ontologies/2016/02/culturalHeritageConservation/NGA#mountCondition
nga:mountCondition rdf:type owl:DatatypeProperty ;
                   rdfs:subPropertyOf chc:condition ;
                   rdfs:range xsd:string ;
                   dc:creator "Lidiya Dimitrova"@en ;
                   rdfs:label "Mount Condition"@en ;
                   skos:definition "Description of the condition of the mount of the cultural object."@en .


###  http://www.sirma.com/ontologies/2016/02/culturalHeritageConservation/NGA#mountDescription
nga:mountDescription rdf:type owl:DatatypeProperty ;
                     rdfs:domain chc:CulturalObject ;
                     rdfs:range xsd:string ;
                     dc:creator "Lidiya Dimitrova"@en ;
                     rdfs:label "Mount Description"@en ;
                     skos:definition "Text description of the mounting when Art objects is on display."@en .


###  http://www.sirma.com/ontologies/2016/02/culturalHeritageConservation/NGA#numberOfObjects
nga:numberOfObjects rdf:type owl:DatatypeProperty ;
                    rdfs:range xsd:string ;
                    dc:creator "Malvina Makarieva"@en ;
                    rdfs:label "Number of оbjects"@en ;
                    skos:definition "The number of cultural objects involved in the activity."@en .


###  http://www.sirma.com/ontologies/2016/02/culturalHeritageConservation/NGA#objectDepartmentName
nga:objectDepartmentName rdf:type owl:DatatypeProperty ;
                         rdfs:domain chc:CulturalObject ;
                         rdfs:range xsd:string ;
                         dc:creator "Lidiya Dimitrova"@en ;
                         rdfs:label "Object Department"@en ;
                         skos:definition "The object department responsible for the curatorial management and displaying for exhibition but acquisition is done by Registrar office."@en .


###  http://www.sirma.com/ontologies/2016/02/culturalHeritageConservation/NGA#outgoingLoanNumber
nga:outgoingLoanNumber rdf:type owl:DatatypeProperty ;
                       rdfs:range xsd:string ;
                       dc:creator "Lidiya Dimitrova" ;
                       rdfs:label "Outgoing Loan Number" ;
                       skos:definition "Unique  number that is assigned to a Loan for an Exhibition Outside of the organization and can have one or more objects." .


###  http://www.sirma.com/ontologies/2016/02/culturalHeritageConservation/NGA#overallConditionAppraisal
nga:overallConditionAppraisal rdf:type owl:DatatypeProperty ;
                              rdfs:subPropertyOf chc:condition ;
                              rdfs:range xsd:string ;
                              dc:creator "Lidiya Dimitrova"@en ;
                              rdfs:label "Overall condition appraisal"@en ;
                              skos:definition "General description of the condition of the cultural object."@en .


###  http://www.sirma.com/ontologies/2016/02/culturalHeritageConservation/NGA#ownerNames
nga:ownerNames rdf:type owl:DatatypeProperty ;
               rdfs:domain chc:CulturalObject ;
               rdfs:range xsd:string ;
               dc:creator "Lidiya Dimitrova"@en ;
               rdfs:label "Owner/Custodian"@en ;
               skos:definition "The owner (person or organization) of a cultural object. The cultural object is not always a museum's possession."@en .


###  http://www.sirma.com/ontologies/2016/02/culturalHeritageConservation/NGA#packingRequirements
nga:packingRequirements rdf:type owl:DatatypeProperty ;
                        rdfs:domain chc:CulturalObject ;
                        rdfs:range xsd:string ;
                        dc:creator "Lidiya Dimitrova"@en ;
                        rdfs:label "Packing Notes"@en ;
                        skos:definition "Description of any special packing notes/instructions for movement or transport  for this cultural object."@en .


###  http://www.sirma.com/ontologies/2016/02/culturalHeritageConservation/NGA#paintLayersCondition
nga:paintLayersCondition rdf:type owl:DatatypeProperty ;
                         rdfs:subPropertyOf chc:condition ;
                         rdfs:range xsd:string ;
                         dc:creator "Lidiya Dimitrova"@en ;
                         rdfs:label "Paint Layers Condition"@en ;
                         skos:definition "Description of the paint layer or design condition."@en .


###  http://www.sirma.com/ontologies/2016/02/culturalHeritageConservation/NGA#paintLayersDescription
nga:paintLayersDescription rdf:type owl:DatatypeProperty ;
                           rdfs:domain chc:CulturalObject ;
                           rdfs:range xsd:string ;
                           dc:creator "Lidiya Dimitrova"@en ;
                           rdfs:label "Paint Layers Description"@en ;
                           skos:definition "Technical description of the paint layer or design construction."@en .


###  http://www.sirma.com/ontologies/2016/02/culturalHeritageConservation/NGA#photographerName
nga:photographerName rdf:type owl:DatatypeProperty ;
                     rdfs:range xsd:string ;
                     dc:creator "Lidiya Dimitrova"@en ;
                     rdfs:label "Photographer"@en ;
                     skos:definition "Name of the photographer"@en .


###  http://www.sirma.com/ontologies/2016/02/culturalHeritageConservation/NGA#physicalDimensions
nga:physicalDimensions rdf:type owl:DatatypeProperty ;
                       rdfs:domain chc:CulturalObject ;
                       rdfs:range xsd:string ;
                       dc:creator "Kiril Penev"@en ;
                       rdfs:label "Base Physical Dimensions"@en ;
                       skos:definition "The physical attributes of the object without matte and/or frame. Both US and metric. Can be complex with multi-component or 3-dimensional objects. Includes weight and other measures of the physical attributes of objects and their components."@en .


###  http://www.sirma.com/ontologies/2016/02/culturalHeritageConservation/NGA#physicalLocation
nga:physicalLocation rdf:type owl:DatatypeProperty ;
                     rdfs:range xsd:string ;
                     dc:creator "Lidiya Dimitrova"@en ;
                     rdfs:label "Physical Location"@en ;
                     skos:definition "Physical location of the sample so that someone could lay their hands on such as drawer number."@en .


###  http://www.sirma.com/ontologies/2016/02/culturalHeritageConservation/NGA#portfolioTitle
nga:portfolioTitle rdf:type owl:DatatypeProperty ;
                   rdfs:domain chc:CulturalObject ;
                   rdfs:range xsd:string ;
                   dc:creator "Lidiya Dimitrova" ;
                   rdfs:label "Portfolio/Series"@en ;
                   skos:definition "Indication of a group of works of art created as a group."@en .


###  http://www.sirma.com/ontologies/2016/02/culturalHeritageConservation/NGA#preserverCondition
nga:preserverCondition rdf:type owl:DatatypeProperty ;
                       rdfs:subPropertyOf chc:condition ;
                       rdfs:range xsd:string ;
                       dc:creator "Lidiya Dimitrova"@en ;
                       rdfs:label "Preserver Condition"@en ;
                       skos:definition "Description of the preserver condition."@en .


###  http://www.sirma.com/ontologies/2016/02/culturalHeritageConservation/NGA#preserverDescription
nga:preserverDescription rdf:type owl:DatatypeProperty ;
                         rdfs:domain nga:Photograph ;
                         rdfs:range xsd:string ;
                         dc:creator "Lidiya Dimitrova"@en ;
                         rdfs:label "Preserver Description"@en ;
                         skos:definition "Description of preserver in a cased object."@en .


###  http://www.sirma.com/ontologies/2016/02/culturalHeritageConservation/NGA#primingCondition
nga:primingCondition rdf:type owl:DatatypeProperty ;
                     rdfs:subPropertyOf chc:condition ;
                     rdfs:range xsd:string ;
                     dc:creator "Lidiya Dimitrova"@en ;
                     rdfs:label "Sizing and Ground Condition"@en ;
                     skos:definition "Description of the sizing and ground condition."@en .


###  http://www.sirma.com/ontologies/2016/02/culturalHeritageConservation/NGA#primingDescription
nga:primingDescription rdf:type owl:DatatypeProperty ;
                       rdfs:domain chc:CulturalObject ;
                       rdfs:range xsd:string ;
                       dc:creator "Lidiya Dimitrova" ;
                       rdfs:label "Sizing and Ground Description"@en ;
                       skos:definition "Description of the sizes and/or grounds applied to the primary support."@en .


###  http://www.sirma.com/ontologies/2016/02/culturalHeritageConservation/NGA#productDescription
nga:productDescription rdf:type owl:DatatypeProperty ;
                       rdfs:range xsd:string ;
                       dc:creator "Lidiya Dimitrova"@en ;
                       rdfs:label "Description of Product"@en ;
                       skos:definition "Description of product for analysis."@en .


###  http://www.sirma.com/ontologies/2016/02/culturalHeritageConservation/NGA#provenance
nga:provenance rdf:type owl:DatatypeProperty ;
               rdfs:domain chc:CulturalObject ;
               rdfs:range xsd:string ;
               dc:creator "Lidiya Dimitrova"@en ;
               rdfs:label "Provenance"@en ;
               skos:definition "Historical ownership of an art object."@en .


###  http://www.sirma.com/ontologies/2016/02/culturalHeritageConservation/NGA#publicationDate
nga:publicationDate rdf:type owl:DatatypeProperty ;
                    rdfs:domain chc:CulturalObject ;
                    rdfs:range xsd:string ;
                    dc:creator "Lidiya Dimitrova"@en ;
                    rdfs:label "Publication Date"@en ;
                    skos:definition "Date of publication of the cultural object."@en .


###  http://www.sirma.com/ontologies/2016/02/culturalHeritageConservation/NGA#publicationPlace
nga:publicationPlace rdf:type owl:DatatypeProperty ;
                     rdfs:domain nga:BoundVolume ;
                     rdfs:range xsd:string ;
                     dc:creator "Lidiya Dimitrova" ;
                     rdfs:label "Place of publication"@en ;
                     skos:definition "Identifies the city of publication."@en .


###  http://www.sirma.com/ontologies/2016/02/culturalHeritageConservation/NGA#purpose
nga:purpose rdf:type owl:DatatypeProperty ;
            rdfs:range xsd:string ;
            dc:creator "Malvina Makarieva" ;
            rdfs:label "Purpose"@en ;
            skos:definition "Defies the purpose of the document such as Loan, Exhibition, Travel and ect ."@en .


###  http://www.sirma.com/ontologies/2016/02/culturalHeritageConservation/NGA#relatedObjectClassification
nga:relatedObjectClassification rdf:type owl:DatatypeProperty ;
                                rdfs:range xsd:string ;
                                dc:creator "Malvina Makarieva" ;
                                rdfs:label "Related Object Classification"@en ;
                                skos:definition "Type of object(s) associated with the task."@en .


###  http://www.sirma.com/ontologies/2016/02/culturalHeritageConservation/NGA#reportDate
nga:reportDate rdf:type owl:DatatypeProperty ;
               rdfs:range xsd:dateTime ;
               dc:creator "Lidiya Dimitrova" ;
               rdfs:label "Date of the report"@en ;
               skos:definition "Defines the date of the report. "@en .


###  http://www.sirma.com/ontologies/2016/02/culturalHeritageConservation/NGA#requestNumber
nga:requestNumber rdf:type owl:DatatypeProperty ;
                  rdfs:range xsd:dateTime ;
                  dc:creator "Malvina Makariva" ;
                  rdfs:label "Request number "@en ;
                  skos:definition "The corresponding filemaker pro number . "@en .


###  http://www.sirma.com/ontologies/2016/02/culturalHeritageConservation/NGA#sampleCondition
nga:sampleCondition rdf:type owl:DatatypeProperty ;
                    rdfs:subPropertyOf chc:condition ;
                    rdfs:range xsd:string ;
                    dc:creator "Lidiya Dimitrova" ;
                    rdfs:label "Sample Condition"@en ;
                    skos:definition "Condition of the sample."@en .


###  http://www.sirma.com/ontologies/2016/02/culturalHeritageConservation/NGA#sampleMaterialsIdentified
nga:sampleMaterialsIdentified rdf:type owl:DatatypeProperty ;
                              rdfs:range xsd:string ;
                              dc:creator "Lidiya Dimitrova"@en ;
                              rdfs:label "Materials  identified"@en ;
                              skos:definition "Materials identified in the analysis of the sample: for example \"chrome yellow in linseed oil."@en .


###  http://www.sirma.com/ontologies/2016/02/culturalHeritageConservation/NGA#sampleSite
nga:sampleSite rdf:type owl:DatatypeProperty ;
               rdfs:range xsd:string ;
               dc:creator "Lidiya Dimitrova" ;
               rdfs:label "Sample Site"@en ;
               skos:definition "Location of the spot where the sample was taken: coordinates \"up\" and \"left\" or \"from right hand of the sitter\"."@en .


###  http://www.sirma.com/ontologies/2016/02/culturalHeritageConservation/NGA#samplingDate
nga:samplingDate rdf:type owl:DatatypeProperty ;
                 rdfs:range xsd:dateTime ;
                 dc:creator "Lidiya Dimitrova" ;
                 rdfs:label "Date taken"@en ;
                 skos:definition "Date on which the sample was taken."@en .


###  http://www.sirma.com/ontologies/2016/02/culturalHeritageConservation/NGA#samplingDateRequested
nga:samplingDateRequested rdf:type owl:DatatypeProperty ;
                          rdfs:range xsd:dateTime ;
                          dc:creator "Lidiya Dimitrova" ;
                          rdfs:label "Date Requested"@en ;
                          skos:definition "The data on which sample analysis is requested"@en .


###  http://www.sirma.com/ontologies/2016/02/culturalHeritageConservation/NGA#samplingReason
nga:samplingReason rdf:type owl:DatatypeProperty ;
                   rdfs:range xsd:string ;
                   dc:creator "Lidiya Dimitrova" ;
                   rdfs:label "Reason for sampling"@en ;
                   skos:definition "Reason for sampling/motivation for sampling"@en .


###  http://www.sirma.com/ontologies/2016/02/culturalHeritageConservation/NGA#secondarySupportCondition
nga:secondarySupportCondition rdf:type owl:DatatypeProperty ;
                              rdfs:subPropertyOf chc:condition ;
                              rdfs:range xsd:string ;
                              dc:creator "Lidiya Dimitrova"@en ;
                              rdfs:label "Secondary Support Condition"@en ;
                              skos:definition "Description of any secondary support (stretcher, lining canvas, etc). The secondary support is  second, newer than the original, support for the cultural object. "@en .


###  http://www.sirma.com/ontologies/2016/02/culturalHeritageConservation/NGA#secondarySupportDescription
nga:secondarySupportDescription rdf:type owl:DatatypeProperty ;
                                rdfs:domain chc:CulturalObject ;
                                rdfs:range xsd:string ;
                                dc:creator "Lidiya Dimitrova"@en ;
                                rdfs:label "Secondary support"@en ;
                                skos:definition "Description of any secondary support (stretcher, lining canvas, etc). The secondary support is  second, newer than the original, support for the cultural object.  The support can be: For photograph -  glued or attached layer or material for support. For drawing -  thick laid paper. For painting - stretcher, lining canvas, etc."@en .


###  http://www.sirma.com/ontologies/2016/02/culturalHeritageConservation/NGA#spectralRange
nga:spectralRange rdf:type owl:DatatypeProperty ;
                  rdfs:range xsd:string ;
                  dc:creator "Lidiya Dimitrova"@en ;
                  rdfs:label "Spectral Range"@en ;
                  skos:definition "The type of light used for the photograph to be taken."@en .


###  http://www.sirma.com/ontologies/2016/02/culturalHeritageConservation/NGA#structureCondition
nga:structureCondition rdf:type owl:DatatypeProperty ;
                       rdfs:subPropertyOf chc:condition ;
                       rdfs:range xsd:string ;
                       dc:creator "Lidiya Dimitrova"@en ;
                       rdfs:label "Structural Condition"@en ;
                       skos:definition "Description of the condition of the structure of the cultural object."@en .


###  http://www.sirma.com/ontologies/2016/02/culturalHeritageConservation/NGA#structureDescription
nga:structureDescription rdf:type owl:DatatypeProperty ;
                         rdfs:domain chc:CulturalObject ;
                         rdfs:range xsd:string ;
                         dc:creator "Lidiya Dimitrova"@en ;
                         rdfs:label "Structure Description"@en ;
                         skos:definition "Description of the structure of the cultural objects - material used and the relationship between them."@en .


###  http://www.sirma.com/ontologies/2016/02/culturalHeritageConservation/NGA#style
nga:style rdf:type owl:DatatypeProperty ;
          rdfs:domain nga:Frame ;
          rdfs:range xsd:string ;
          dc:creator "Lidiya Dimitrova"@en ;
          rdfs:label "Style"@en ;
          skos:definition "A way of Painting, drawing, building, composing, etc. Characteristic of a particular period, place, person or movement."@en .


###  http://www.sirma.com/ontologies/2016/02/culturalHeritageConservation/NGA#subClassification
nga:subClassification rdf:type owl:DatatypeProperty ;
                      rdfs:range xsd:string ;
                      dc:creator "Lidiya Dimitrova"@en ;
                      rdfs:label "Sub-Classification"@en ;
                      skos:definition "Object sub-classification."@en .


###  http://www.sirma.com/ontologies/2016/02/culturalHeritageConservation/NGA#substrateCondition
nga:substrateCondition rdf:type owl:DatatypeProperty ;
                       rdfs:subPropertyOf chc:condition ;
                       rdfs:range xsd:string ;
                       dc:creator "Lidiya Dimitrova"@en ;
                       rdfs:label "Substrate Condition"@en ;
                       skos:definition "Description of the cultural object substrate. For decorative art cultural object this is is a layer before the surface, for a photograph this is the primary or underlying material on which other materials, such as ink, coating, paint, or treatment, are applied"@en .


###  http://www.sirma.com/ontologies/2016/02/culturalHeritageConservation/NGA#substrateDescription
nga:substrateDescription rdf:type owl:DatatypeProperty ;
                         rdfs:domain chc:CulturalObject ;
                         rdfs:range xsd:string ;
                         dc:creator "Lidiya Dimitrova"@en ;
                         rdfs:label "Substrate Description"@en ;
                         skos:definition "Description of the cultural object substrate. For decorative art cultural object this is is a layer before the surface, for a photograph this is the primary or underlying material on which other materials, such as ink, coating, paint, or treatment, are applied"@en .


###  http://www.sirma.com/ontologies/2016/02/culturalHeritageConservation/NGA#supportCondition
nga:supportCondition rdf:type owl:DatatypeProperty ;
                     rdfs:subPropertyOf chc:condition ;
                     rdfs:range xsd:string ;
                     dc:creator "Lidiya Dimitrova"@en ;
                     rdfs:label "Support Condition"@en ;
                     skos:definition "Description of the condition of the paper support. Example: torn and delaminating  chine colle"@en .


###  http://www.sirma.com/ontologies/2016/02/culturalHeritageConservation/NGA#supportDescription
nga:supportDescription rdf:type owl:DatatypeProperty ;
                       rdfs:domain chc:CulturalObject ;
                       rdfs:range xsd:string ;
                       dc:creator "Lidiya Dimitrova"@en ;
                       rdfs:label "Support Description"@en ;
                       skos:definition "Description of the support.  For painting it can be the canvas, paper, etc. For photograph it is the primary or underlying material on which other materials, such as ink, binder, coating, paint, or treatment, are applied: Paper(negative), Iron(tin type),glass(clodian, ambrotype), Film, Copper(silver dagurreotype), Polo-ride"@en .


###  http://www.sirma.com/ontologies/2016/02/culturalHeritageConservation/NGA#surfaceCoatingCondition
nga:surfaceCoatingCondition rdf:type owl:DatatypeProperty ;
                            rdfs:subPropertyOf chc:condition ;
                            rdfs:range xsd:string ;
                            dc:creator "Lidiya Dimitrova"@en ;
                            rdfs:label "Surface Coating Condition"@en ;
                            skos:definition "Description of the surface coating condition."@en .


###  http://www.sirma.com/ontologies/2016/02/culturalHeritageConservation/NGA#surfaceCoatingMaterial
nga:surfaceCoatingMaterial rdf:type owl:DatatypeProperty ;
                           rdfs:domain chc:CulturalObject ;
                           rdfs:range xsd:string ;
                           dc:creator "Lidiya Dimitrova"@en ;
                           rdfs:label "Surface Coating Description"@en ;
                           skos:definition "Description of the surface coating material (such as natural resins, waxes, gelatin, albumen, or anti-halation layer for film)."@en .


###  http://www.sirma.com/ontologies/2016/02/culturalHeritageConservation/NGA#surfaceCondition
nga:surfaceCondition rdf:type owl:DatatypeProperty ;
                     rdfs:subPropertyOf chc:condition ;
                     rdfs:range xsd:string ;
                     dc:creator "Lidiya DImitrova"@en ;
                     rdfs:label "Surface Condition "@en ;
                     skos:definition "Description of the condition of the surface of the cultural object."@en .


###  http://www.sirma.com/ontologies/2016/02/culturalHeritageConservation/NGA#surfaceDescription
nga:surfaceDescription rdf:type owl:DatatypeProperty ;
                       rdfs:domain chc:CulturalObject ;
                       rdfs:range xsd:string ;
                       dc:creator "Lidiya DImitrova"@en ;
                       rdfs:label "Surface Description"@en ;
                       skos:definition "Description of the surface of an art objects. For sculpture this is the outside part or uppermost layer of something (often used when describing its texture, form, or extent)."@en .


###  http://www.sirma.com/ontologies/2016/02/culturalHeritageConservation/NGA#technique
nga:technique rdf:type owl:DatatypeProperty ;
              rdfs:range xsd:string ;
              dc:creator "Lidiya DImitrova"@en ;
              rdfs:label "Technique"@en ;
              skos:definition "Description of the technique with which the sample was taken."@en .


###  http://www.sirma.com/ontologies/2016/02/culturalHeritageConservation/NGA#tradeName
nga:tradeName rdf:type owl:DatatypeProperty ;
              rdfs:range xsd:string ;
              dc:creator "Lidiya Dimitrova"@en ;
              rdfs:label "Trade Name"@en ;
              skos:definition "Trade name of the product."@en .


###  http://www.sirma.com/ontologies/2016/02/culturalHeritageConservation/NGA#treatedObjects
nga:treatedObjects rdf:type owl:DatatypeProperty ;
                   rdfs:range xsd:string ;
                   dc:creator "Malvina Makarieva"@en ;
                   rdfs:label "Single/Multiple"@en ;
                   skos:definition "Indefies if the the document is related to single or multiple objects."@en .


###  http://www.sirma.com/ontologies/2016/02/culturalHeritageConservation/NGA#treatmentType
nga:treatmentType rdf:type owl:DatatypeProperty ;
                  rdfs:range xsd:string ;
                  dc:creator "Lidiya Dimitrova"@en ;
                  rdfs:label "Treatment"@en ;
                  skos:definition "Indicates if the treatment is minor or major."@en .


###  http://www.sirma.com/ontologies/2016/02/culturalHeritageConservation/NGA#variableComponents
nga:variableComponents rdf:type owl:DatatypeProperty ;
                       rdfs:domain nga:Photograph ;
                       rdfs:range xsd:string ;
                       dc:creator "Lidiya Dimitrova"@en ;
                       rdfs:label "Variable Components"@en ;
                       skos:definition "Components that may be changed, such as a projector type, or may not be included in a given installation."@en .


###  http://www.sirma.com/ontologies/2016/02/culturalHeritageConservation/NGA#vendorID
nga:vendorID rdf:type owl:DatatypeProperty ;
             rdfs:domain nga:Frame ;
             rdfs:range xsd:string ;
             dc:creator "Lidiya Dimitrova"@en ;
             rdfs:label "Vendor-ID"@en ;
             skos:definition "The identifier of the Vendor who sold the Frame."@en .


###  http://www.sirma.com/ontologies/2016/02/culturalHeritageConservation/NGA#vendorName
nga:vendorName rdf:type owl:DatatypeProperty ;
               rdfs:range xsd:string ;
               dc:creator "Lidiya Dimitrova"@en ;
               rdfs:label "Vendor/Vendor Manufacturer"@en ;
               skos:definition "The name of the Vendor who sold the Frame."@en .


###  http://www.sirma.com/ontologies/2016/02/culturalHeritageConservation/NGA#viewType
nga:viewType rdf:type owl:DatatypeProperty ;
             rdfs:range xsd:string ;
             dc:creator "Lidiya Dimitrova"@en ;
             rdfs:label "View Type"@en ;
             skos:definition "Describes the vantage point of the image.."@en .


###  http://www.sirma.com/ontologies/2016/02/culturalHeritageConservation/NGA#volume
nga:volume rdf:type owl:DatatypeProperty ;
           rdfs:domain chc:CulturalObject ;
           rdfs:range xsd:string ;
           dc:creator "Lidiya Dimitrova" ;
           rdfs:label "Volume"@en ;
           skos:definition "The number of the volume in a set."@en .


###  http://www.sirma.com/ontologies/2016/02/culturalHeritageConservation/NGA#volumeLanguage
nga:volumeLanguage rdf:type owl:DatatypeProperty ;
                   rdfs:domain chc:CulturalObject ;
                   rdfs:range xsd:string ;
                   dc:creator "Lidiya Dimitrova" ;
                   rdfs:label "Language"@en ;
                   skos:definition "The number of the volume, especially in a set."@en .


###  http://www.sirma.com/ontologies/2016/02/culturalHeritageConservation/NGA#watermarks
nga:watermarks rdf:type owl:DatatypeProperty ;
               rdfs:domain chc:CulturalObject ;
               rdfs:range xsd:string ;
               dc:creator "Lidiya Dimitrova"@en ;
               rdfs:label "Watermarks" ;
               skos:definition "Description of any watermarks evident in the paper/support."@en .


###  http://www.sirma.com/ontologies/2016/02/culturalHeritageConservation/NGA#weaveDescription
nga:weaveDescription rdf:type owl:DatatypeProperty ;
                     rdfs:domain chc:CulturalObject ;
                     rdfs:range xsd:string ;
                     dc:creator "Lidiya Dimitrova"@en ;
                     rdfs:label "Weave Description"@en ;
                     skos:definition "A text description of different weave characteristics in the cultural object, making surface and substrate at the same time in textile or carpet. Might include fiber type, plys, spin, dyes used, etc."@en .


###  http://www.sirma.com/ontologies/2016/02/culturalHeritageConservation/NGA#weight
nga:weight rdf:type owl:DatatypeProperty ;
           rdfs:domain chc:CulturalObject ;
           rdfs:range xsd:string ;
           dc:creator "Lidiya Dimitrova"@en ;
           rdfs:label "Weight"@en ;
           skos:definition "Cultural object weight"@en .


#################################################################
#    Classes
#################################################################

###  http://www.sirma.com/ontologies/2016/02/culturalHeritageConservation#CulturalObject
chc:CulturalObject emf:isSearchable "true"^^xsd:boolean .


###  http://www.sirma.com/ontologies/2016/02/culturalHeritageConservation/NGA#BoundVolume
nga:BoundVolume rdf:type owl:Class ;
                rdfs:subClassOf chc:CulturalObject ;
                emf:classCategory "culturalobject" ;
                emf:definitionId "objectinstance" ;
                emf:isCreateable "true"^^xsd:boolean ;
                emf:isPartOfObjectLibrary "true"^^xsd:boolean ;
                emf:isSearchable "true"^^xsd:boolean ;
                dc:creator "Lidiya Dimitrova"@en ;
                sec:allowInheritLibraryPermissions "true"^^xsd:boolean ;
                sec:allowInheritParentPermissions "false"^^xsd:boolean ;
                rdfs:label "Bound Volume"@en ;
                skos:definition "A volume is a bound collection of printed pages such as a book."@en .


###  http://www.sirma.com/ontologies/2016/02/culturalHeritageConservation/NGA#DecorativeArt
nga:DecorativeArt rdf:type owl:Class ;
                  rdfs:subClassOf chc:CulturalObject ;
                  emf:classCategory "culturalobject" ;
                  emf:definitionId "objectinstance" ;
                  emf:isCreateable "true"^^xsd:boolean ;
                  emf:isPartOfObjectLibrary "true"^^xsd:boolean ;
                  emf:isSearchable "true"^^xsd:boolean ;
                  dc:creator "Lidiya Dimitrova"@en ;
                  sec:allowInheritLibraryPermissions "true"^^xsd:boolean ;
                  sec:allowInheritParentPermissions "false"^^xsd:boolean ;
                  rdfs:label "Decorative Art"@en ;
                  skos:definition "The decorative arts are arts or crafts concerned with the design and manufacture of beautiful objects that are also functional. It includes interior design, but not usually architecture . Examples include things like candle sticks, furniture, porcelain dinnerware, etc."@en .


###  http://www.sirma.com/ontologies/2016/02/culturalHeritageConservation/NGA#Drawing
nga:Drawing rdf:type owl:Class ;
            rdfs:subClassOf chc:CulturalObject ;
            emf:classCategory "culturalobject" ;
            emf:definitionId "objectinstance" ;
            emf:isCreateable "true"^^xsd:boolean ;
            emf:isPartOfObjectLibrary "true"^^xsd:boolean ;
            emf:isSearchable "true"^^xsd:boolean ;
            dc:creator "Kiril Penev"@en ;
            sec:allowInheritLibraryPermissions "true"^^xsd:boolean ;
            sec:allowInheritParentPermissions "false"^^xsd:boolean ;
            rdfs:label "Drawing"@en ;
            skos:definition "Drawing is a form of visual art that makes use of any number of drawing instruments to mark a two-dimensional medium. Instruments used include graphite pencils, pen and ink, inked brushes, wax color pencils, crayons, charcoal, chalk, pastels, various kinds of erasers, markers, styluses, and various metals (such as silverpoint) (Wikipedia)"@en .


###  http://www.sirma.com/ontologies/2016/02/culturalHeritageConservation/NGA#Ephemera
nga:Ephemera rdf:type owl:Class ;
             rdfs:subClassOf chc:CulturalObject ;
             emf:classCategory "culturalobject" ;
             emf:definitionId "objectinstance" ;
             emf:isCreateable "true"^^xsd:boolean ;
             emf:isPartOfObjectLibrary "true"^^xsd:boolean ;
             emf:isSearchable "true"^^xsd:boolean ;
             dc:creator "Lidiya Dimitrova" ;
             sec:allowInheritLibraryPermissions "true"^^xsd:boolean ;
             sec:allowInheritParentPermissions "false"^^xsd:boolean ;
             rdfs:label "Ephemera" ;
             skos:definition "Ephemera are any transitory written or printed matter meant for eventual repression (or not meant to be retained or preserved). However in the museum or archives context, ephemera must be preserved and accounted for." .


###  http://www.sirma.com/ontologies/2016/02/culturalHeritageConservation/NGA#Frame
nga:Frame rdf:type owl:Class ;
          rdfs:subClassOf chc:CulturalObject ;
          emf:classCategory "culturalobject" ;
          emf:definitionId "objectinstance" ;
          emf:isCreateable "true"^^xsd:boolean ;
          emf:isPartOfObjectLibrary "true"^^xsd:boolean ;
          emf:isSearchable "true"^^xsd:boolean ;
          dc:creator "Lidiya Dimitrova"@en ;
          sec:allowInheritLibraryPermissions "true"^^xsd:boolean ;
          sec:allowInheritParentPermissions "false"^^xsd:boolean ;
          rdfs:label "Frame"@en ;
          skos:definition "A frame is a decorative molding that typically is attached to a painting or other cultural object especially when that cultural object is displayed. It typically surrounds and covers the edges of the cultural object. It is typically made of wood/plaster/gold leaf, but can be any material."@en .


###  http://www.sirma.com/ontologies/2016/02/culturalHeritageConservation/NGA#MediaArt
nga:MediaArt rdf:type owl:Class ;
             rdfs:subClassOf chc:CulturalObject ;
             emf:classCategory "culturalobject" ;
             emf:definitionId "objectinstance" ;
             emf:isCreateable "true"^^xsd:boolean ;
             emf:isPartOfObjectLibrary "true"^^xsd:boolean ;
             emf:isSearchable "true"^^xsd:boolean ;
             dc:creator "Lidiya Dimitrova"@en ;
             sec:allowInheritLibraryPermissions "true"^^xsd:boolean ;
             sec:allowInheritParentPermissions "false"^^xsd:boolean ;
             rdfs:label "Media Art"@en ;
             skos:definition "Media art is a genre that encompasses artworks created with new media technologies, including digital art, computer animation, computer graphics, virtual art, internet art, interactive art, video games, computer robotics, 3-D printing, and art as biotechnology. It can also include film if not represented elsewhere."@en .


###  http://www.sirma.com/ontologies/2016/02/culturalHeritageConservation/NGA#Painting
nga:Painting rdf:type owl:Class ;
             rdfs:subClassOf chc:CulturalObject ;
             emf:classCategory "culturalobject" ;
             emf:definitionId "objectinstance" ;
             emf:isCreateable "true"^^xsd:boolean ;
             emf:isPartOfObjectLibrary "true"^^xsd:boolean ;
             emf:isSearchable "true"^^xsd:boolean ;
             dc:creator "Kiril Penev"@en ;
             sec:allowInheritLibraryPermissions "true"^^xsd:boolean ;
             sec:allowInheritParentPermissions "false"^^xsd:boolean ;
             rdfs:label "Painting"@en ;
             skos:definition "Painting is the practice of applying paint, pigment, color or other medium to a surface (support base). The medium is commonly applied to the base with a brush but other implements, such as knives, sponges, and airbrushes, can be used. In art, the term painting describes both the act and the result of the action. However, painting is also used outside of art as a common trade among craftsmen and builders. Paintings may have for their support such surfaces as walls, paper, canvas, wood, glass, lacquer, clay, leaf, copper or concrete, and may incorporate multiple other materials including sand, clay, paper, gold leaf as well as objects. (Wikipedia)"@en .


###  http://www.sirma.com/ontologies/2016/02/culturalHeritageConservation/NGA#Photograph
nga:Photograph rdf:type owl:Class ;
               rdfs:subClassOf chc:CulturalObject ;
               emf:classCategory "culturalobject" ;
               emf:definitionId "objectinstance" ;
               emf:isCreateable "true"^^xsd:boolean ;
               emf:isPartOfObjectLibrary "true"^^xsd:boolean ;
               emf:isSearchable "true"^^xsd:boolean ;
               dc:creator "Kiril Penev"@en ;
               sec:allowInheritLibraryPermissions "true"^^xsd:boolean ;
               sec:allowInheritParentPermissions "false"^^xsd:boolean ;
               rdfs:label "Photograph"@en ;
               skos:definition "A photograph or photo is an image created by light falling on a light-sensitive surface, usually photographic film or an electronic image such as a CCD or a CMOS chip. Most photographs are created using a camera, which uses a lens to focus the scene's visible wavelengths of light into a reproduction of what the human eye would see. (Wikipedia)"@en .


###  http://www.sirma.com/ontologies/2016/02/culturalHeritageConservation/NGA#Portfolio
nga:Portfolio rdf:type owl:Class ;
              rdfs:subClassOf chc:CulturalObject ;
              emf:classCategory "culturalobject" ;
              emf:definitionId "objectinstance" ;
              emf:isCreateable "true"^^xsd:boolean ;
              emf:isPartOfObjectLibrary "true"^^xsd:boolean ;
              emf:isSearchable "true"^^xsd:boolean ;
              dc:creator "Lidiya Dimitrova"@en ;
              sec:allowInheritLibraryPermissions "true"^^xsd:boolean ;
              sec:allowInheritParentPermissions "false"^^xsd:boolean ;
              rdfs:label "Portfolio"@en ;
              skos:definition "A portfolio is an edited collection of artwork. It usually has a cover or housing to keep the collection together. "@en .


###  http://www.sirma.com/ontologies/2016/02/culturalHeritageConservation/NGA#Print
nga:Print rdf:type owl:Class ;
          rdfs:subClassOf chc:CulturalObject ;
          emf:classCategory "culturalobject" ;
          emf:definitionId "objectinstance" ;
          emf:isCreateable "true"^^xsd:boolean ;
          emf:isPartOfObjectLibrary "true"^^xsd:boolean ;
          emf:isSearchable "true"^^xsd:boolean ;
          dc:creator "Kiril Penev"@en ;
          sec:allowInheritLibraryPermissions "true"^^xsd:boolean ;
          sec:allowInheritParentPermissions "false"^^xsd:boolean ;
          rdfs:label "Print"@en ;
          skos:definition """A picture or design printed from a block or plate or copied from a painting by photography.
A piece of fabric or clothing with a decorative colored pattern or design printed on it."""@en .


###  http://www.sirma.com/ontologies/2016/02/culturalHeritageConservation/NGA#Sculpture
nga:Sculpture rdf:type owl:Class ;
              rdfs:subClassOf chc:CulturalObject ;
              emf:classCategory "culturalobject" ;
              emf:definitionId "objectinstance" ;
              emf:isCreateable "true"^^xsd:boolean ;
              emf:isPartOfObjectLibrary "true"^^xsd:boolean ;
              emf:isSearchable "true"^^xsd:boolean ;
              dc:creator "Kiril Penev"@en ;
              sec:allowInheritLibraryPermissions "true"^^xsd:boolean ;
              sec:allowInheritParentPermissions "false"^^xsd:boolean ;
              rdfs:label "Sculpture"@en ;
              skos:definition "Sculpture is the branch of the visual arts that operates in three dimensions, and one of the plastic arts. Durable sculptural processes originally used carving (the removal of material) and modelling (the addition of material, as clay), in stone, metal, ceramics, wood and other materials but, since modernism, shifts in sculptural process led to an almost complete freedom of materials and process. A wide variety of materials may be worked by removal such as carving, assembled by welding or modelling, or molded, or cast. (Wikipedia)"@en .


###  http://www.sirma.com/ontologies/2016/02/culturalHeritageConservation/NGA#TechnicalMaterial
nga:TechnicalMaterial rdf:type owl:Class ;
                      rdfs:subClassOf chc:CulturalObject ;
                      emf:classCategory "culturalobject" ;
                      emf:definitionId "objectinstance" ;
                      emf:isCreateable "true"^^xsd:boolean ;
                      emf:isPartOfObjectLibrary "true"^^xsd:boolean ;
                      emf:isSearchable "true"^^xsd:boolean ;
                      dc:creator "Lidiya Dimitrova"@en ;
                      sec:allowInheritLibraryPermissions "true"^^xsd:boolean ;
                      sec:allowInheritParentPermissions "false"^^xsd:boolean ;
                      rdfs:label "Technical Material"@en ;
                      skos:definition "Technical Material (in the context of the NGA's collection management system (TMS)) are accessioned cultural objects that are related to the production of works of art. The best example of these types of materials are metal plates, usually copper, that have been etched or engraved by the artist in order to make a series of prints on paper. Another example could be a mold that an artist made to cast a series of three dimensional sculptures."@en .


#################################################################
#    Annotations
#################################################################

emf:hasAssignee sec:autoAssignPermissionRole "COLLABORATOR" ;
                sec:autoAssignParentPermissionRole "CONTRIBUTOR" .


emf:hasPrimaryImage emf:isSearchable "true"^^xsd:boolean .


emf:hasWatcher sec:autoAssignPermissionRole "CONSUMER" .


emf:isPrimaryImageOf emf:isSearchable "true"^^xsd:boolean .


emf:processedBy emf:isSearchable "true"^^xsd:boolean .


emf:processes emf:isSearchable "true"^^xsd:boolean .


ptop:hasParticipant sec:autoAssignPermissionRole "COLLABORATOR" ;
                    sec:autoAssignParentPermissionRole "CONTRIBUTOR" ;
                    emf:isSearchable "true"^^xsd:boolean ;
                    emf:auditEvent "+addHasParticipant|-removeHasParticipant|changeHasParticipant" .


ptop:involvedIn emf:auditEvent "+addInvolvedIn|-removeInvolvedIn|changeInvolvedIn" ;
                emf:isSearchable "true"^^xsd:boolean .


chc:ConservationActivity emf:isCreateable "true"^^xsd:boolean ;
                         emf:isSearchable "true"^^xsd:boolean ;
                         sec:allowInheritParentPermissions "false"^^xsd:boolean ;
                         emf:isPartOfObjectLibrary "true"^^xsd:boolean ;
                         sec:allowInheritLibraryPermissions "true"^^xsd:boolean .


chc:Sample emf:isCreateable "true"^^xsd:boolean ;
           emf:isPartOfObjectLibrary "true"^^xsd:boolean ;
           emf:isSearchable "true"^^xsd:boolean ;
           sec:allowInheritLibraryPermissions "true"^^xsd:boolean ;
           sec:allowInheritParentPermissions "false"^^xsd:boolean .


chc:approvedBy sec:autoAssignPermissionRole "COLLABORATOR" ;
               sec:autoAssignParentPermissionRole "CONSUMER" ;
               emf:isSearchable "true"^^xsd:boolean .


chc:attachmentOf emf:isSearchable "true"^^xsd:boolean .


chc:depicts emf:isSearchable "true"^^xsd:boolean .


chc:documents emf:isSearchable "true"^^xsd:boolean .


chc:duplicates emf:isSearchable "true"^^xsd:boolean .


chc:hasApproved emf:isSearchable "true"^^xsd:boolean .


chc:hasAttachment emf:isSearchable "true"^^xsd:boolean .


chc:hasAuthor emf:isSearchable "true"^^xsd:boolean ;
              sec:autoAssignParentPermissionRole "CONSUMER" ;
              sec:autoAssignPermissionRole "MANAGER" .


chc:hasDepiction emf:isSearchable "true"^^xsd:boolean .


chc:hasSample emf:isSearchable "true"^^xsd:boolean .


chc:hasSupervisor sec:autoAssignParentPermissionRole "CONTRIBUTOR" ;
                  emf:isSearchable "true"^^xsd:boolean ;
                  sec:autoAssignPermissionRole "COLLABORATOR" .


chc:isAuthorOf emf:isSearchable "true"^^xsd:boolean .


chc:isDocumentedIn emf:isSearchable "true"^^xsd:boolean .


chc:isSupervisorOf emf:isSearchable "true"^^xsd:boolean .


chc:isTakenFrom emf:isSearchable "true"^^xsd:boolean .


###  Generated by the OWL API (version 4.2.8.20170104-2310) https://github.com/owlcs/owlapi
