@prefix : <http://www.semanticweb.org/owl/owlapi/turtle#> .
@prefix dc: <http://purl.org/dc/elements/1.1/> .
@prefix chc: <http://www.sirma.com/ontologies/2016/02/culturalHeritageConservation#> .
@prefix emf: <http://ittruse.ittbg.com/ontology/enterpriseManagementFramework#> .
@prefix owl: <http://www.w3.org/2002/07/owl#> .
@prefix rdf: <http://www.w3.org/1999/02/22-rdf-syntax-ns#> .
@prefix sec: <http://www.sirma.com/ontologies/2014/11/security#> .
@prefix smk: <http://www.sirma.com/ontologies/2016/02/culturalHeritageConservation/SMK#> .
@prefix xml: <http://www.w3.org/XML/1998/namespace> .
@prefix xsd: <http://www.w3.org/2001/XMLSchema#> .
@prefix ptop: <http://www.ontotext.com/proton/protontop#> .
@prefix rdfs: <http://www.w3.org/2000/01/rdf-schema#> .
@prefix skos: <http://www.w3.org/2004/02/skos/core#> .
@prefix dcterms: <http://purl.org/dc/terms/> .
@base <http://www.sirma.com/ontologies/2016/02/culturalHeritageConservation/SMK> .

<http://www.sirma.com/ontologies/2016/02/culturalHeritageConservation/SMK> rdf:type owl:Ontology ;
                                                                            owl:imports <http://www.sirma.com/ontologies/2016/02/culturalHeritageConservation> ;
                                                                            rdfs:comment "SMK Extension of Cultural Heritage Conservation Ontology Model for Conservation Space project"@en ;
                                                                            owl:versionInfo "0.1"@en ;
                                                                            rdfs:label "Extension of Cultural Heritage Conservation Ontology Model for SMK"@en ;
                                                                            dc:creator "Lidiya Dimitrova"@en ;
                                                                            dc:rights "What rights?"@en ;
                                                                            dc:subject "Extension of Cultural Heritage Conservation Ontology Model for SMK"@en .

#################################################################
#    Data properties
#################################################################

###  http://www.sirma.com/ontologies/2016/02/culturalHeritageConservation#condition
chc:condition rdf:type owl:DatatypeProperty .


###  http://www.sirma.com/ontologies/2016/02/culturalHeritageConservation/SMK#acquisitionDate
smk:acquisitionDate rdf:type owl:DatatypeProperty ;
                    rdfs:domain chc:CulturalObject ;
                    rdfs:range xsd:string ;
                    dc:creator "Lidiya Dimitrova"@en ;
                    rdfs:label "Acquisition date"@en ,
                               "Erhvervelsesdatering"@da ;
                    skos:definition "The date the object was acquired to the collections."@en .


###  http://www.sirma.com/ontologies/2016/02/culturalHeritageConservation/SMK#analysisDate
smk:analysisDate rdf:type owl:DatatypeProperty ;
                 rdfs:range xsd:dateTime ;
                 dc:creator "Lidiya Dimitrova"@en ;
                 rdfs:label "Date of analysis"@en ,
                            "Dato for analyse"@da ;
                 skos:definition "Date of any analysis made on the sample."@en .


###  http://www.sirma.com/ontologies/2016/02/culturalHeritageConservation/SMK#artistNames
smk:artistNames rdf:type owl:DatatypeProperty ;
                rdfs:domain chc:CulturalObject ;
                rdfs:range xsd:string ;
                dc:creator "Lidiya Dimitrova"@en ;
                rdfs:label "Artist(s)"@en ,
                           "Kunstner/Producent"@da ;
                skos:definition "An entity primarily responsible for creating an object."@en .


###  http://www.sirma.com/ontologies/2016/02/culturalHeritageConservation/SMK#auxiliarySupport
smk:auxiliarySupport rdf:type owl:DatatypeProperty ;
                     rdfs:domain chc:CulturalObject ;
                     rdfs:range xsd:string ;
                     dc:creator "Lidiya Dimitrova"@en ;
                     rdfs:label "Auxiliary support"@en ,
                                "Bærende underlag"@da ;
                     skos:definition "Technical description of the Auxiliary support."@en .


###  http://www.sirma.com/ontologies/2016/02/culturalHeritageConservation/SMK#auxiliarySupportCondition
smk:auxiliarySupportCondition rdf:type owl:DatatypeProperty ;
                              rdfs:subPropertyOf chc:condition ;
                              rdfs:range xsd:dateTime ;
                              dc:creator "Lidiya Dimitrova"@en ;
                              rdfs:label "Auxiliary support condition"@en ,
                                         "Tilstand bærende underlag"@da ;
                              skos:definition "Technical description of condition of the secondary support."@en .


###  http://www.sirma.com/ontologies/2016/02/culturalHeritageConservation/SMK#auxiliarySupportDistinguishingMarks
smk:auxiliarySupportDistinguishingMarks rdf:type owl:DatatypeProperty ;
                                        rdfs:domain chc:CulturalObject ;
                                        rdfs:range xsd:string ;
                                        dc:creator "Lidiya Dimitrova"@en ;
                                        rdfs:label "Auxiliary support distinguishing marks"@en ,
                                                   "Kendetegn bærende underlag"@da ;
                                        skos:definition "Marks on the auxiliary support that may help to distinguish it."@en .


###  http://www.sirma.com/ontologies/2016/02/culturalHeritageConservation/SMK#baseCondition
smk:baseCondition rdf:type owl:DatatypeProperty ;
                  rdfs:subPropertyOf chc:condition ;
                  rdfs:range xsd:string ;
                  dc:creator "Lidiya Dimitrova"@en ;
                  rdfs:label "Base condition"@en ,
                             "Tilstand sokkel/base"@da ;
                  skos:definition "Description of condition of the base: \"corner damaged\" or mount \"broken\"."@en .


###  http://www.sirma.com/ontologies/2016/02/culturalHeritageConservation/SMK#creationDates
smk:creationDates rdf:type owl:DatatypeProperty ;
                  rdfs:domain chc:CulturalObject ;
                  rdfs:range xsd:string ;
                  dc:creator "Lidiya Dimitrova"@en ;
                  rdfs:label "Create date(s)"@en ,
                             "Datering"@da ;
                  skos:definition "Start/end dates and qualifiers such as \"circa\", \"before\", etc. Can have historical records of former attributions of creation dates."@en .


###  http://www.sirma.com/ontologies/2016/02/culturalHeritageConservation/SMK#currentLocation
smk:currentLocation rdf:type owl:DatatypeProperty ;
                    rdfs:domain chc:CulturalObject ;
                    rdfs:range xsd:string ;
                    dc:creator "Lidiya Dimitrova"@en ;
                    rdfs:label "Aktuel placering"@da ,
                               "Current location"@en ;
                    skos:definition "Indication of the location that the Art Object is physically resides currently."@en .


###  http://www.sirma.com/ontologies/2016/02/culturalHeritageConservation/SMK#currentLocationMoveDate
smk:currentLocationMoveDate rdf:type owl:DatatypeProperty ;
                            rdfs:domain chc:CulturalObject ;
                            rdfs:range xsd:dateTime ;
                            dc:creator "Lidiya Dimitrova"@en ;
                            rdfs:label "Dato placering"@da ,
                                       "Location date"@en ;
                            skos:definition "Date of location movement."@en .


###  http://www.sirma.com/ontologies/2016/02/culturalHeritageConservation/SMK#currentLocationMovePurpose
smk:currentLocationMovePurpose rdf:type owl:DatatypeProperty ;
                               rdfs:domain chc:CulturalObject ;
                               rdfs:range xsd:string ;
                               dc:creator "Lidiya Dimitrova"@en ;
                               rdfs:label "Formål placering"@da ,
                                          "Location type"@en ;
                               skos:definition "Business reason for movement of object."@en .


###  http://www.sirma.com/ontologies/2016/02/culturalHeritageConservation/SMK#dimensionsGross
smk:dimensionsGross rdf:type owl:DatatypeProperty ;
                    rdfs:domain chc:CulturalObject ;
                    rdfs:range xsd:string ;
                    dc:creator "Lidiya Dimitrova"@en ;
                    rdfs:label "Bruttomål"@da ,
                               "Dimensions, gross"@en ;
                    skos:definition "The physical attributes of the object plus attached components, typically a base on sculpture."@en .


###  http://www.sirma.com/ontologies/2016/02/culturalHeritageConservation/SMK#dimensionsNet
smk:dimensionsNet rdf:type owl:DatatypeProperty ;
                  rdfs:domain chc:CulturalObject ;
                  rdfs:range xsd:string ;
                  dc:creator "Lidiya Dimitrova"@en ;
                  rdfs:label "Dimensions, net"@en ,
                             "Nettomål"@da ;
                  skos:definition "The physical attributes of the object without matte and/or frame. Both US and metric. Can be complex with multi-component or 3-dimensional objects."@en .


###  http://www.sirma.com/ontologies/2016/02/culturalHeritageConservation/SMK#documentedCulturalObjectType
smk:documentedCulturalObjectType rdf:type owl:DatatypeProperty ;
                                 rdfs:range xsd:string ;
                                 dc:creator "Malvina Makarieva"@en ;
                                 rdfs:label "Related Cultural Object Type"@en ,
                                            "Værktype relateret værk"@da ;
                                 skos:definition "The type of cultural object related to the document"@en .


###  http://www.sirma.com/ontologies/2016/02/culturalHeritageConservation/SMK#frameCondition
smk:frameCondition rdf:type owl:DatatypeProperty ;
                   rdfs:subPropertyOf chc:condition ;
                   rdfs:range xsd:string ;
                   dc:creator "Lidiya Dimitrova"@en ;
                   rdfs:label "Frame condition"@en ,
                              "Tilstand ramme"@da ;
                   skos:definition "Description of condition of the frame."@en .


###  http://www.sirma.com/ontologies/2016/02/culturalHeritageConservation/SMK#frameDescription
smk:frameDescription rdf:type owl:DatatypeProperty ;
                     rdfs:range xsd:string ;
                     dc:creator "Lidiya Dimitrova"@en ;
                     rdfs:label "Frame information"@en ,
                                "Information ramme"@da ;
                     skos:definition "Technical description of the frame's design and construction."@en .


###  http://www.sirma.com/ontologies/2016/02/culturalHeritageConservation/SMK#frameDistinguishingMarks
smk:frameDistinguishingMarks rdf:type owl:DatatypeProperty ;
                             rdfs:domain chc:CulturalObject ;
                             rdfs:range xsd:string ;
                             dc:creator "Lidiya Dimitrova"@en ;
                             rdfs:label "Frame distinguishing marks"@en ,
                                        "Kendetegn ramme"@da ;
                             skos:definition "Technical description of any marks not related to the image such notations or marks on frame."@en .


###  http://www.sirma.com/ontologies/2016/02/culturalHeritageConservation/SMK#generalConditionAppraisal
smk:generalConditionAppraisal rdf:type owl:DatatypeProperty ;
                              rdfs:subPropertyOf chc:condition ;
                              rdfs:range xsd:string ;
                              dc:creator "Lidiya Dimitrova"@en ;
                              rdfs:label "General condition appraisal"@en ,
                                         "Generel tilstandsvurdering"@da ;
                              skos:definition "General condition appraisal of the media/support of a particular cultural object."@en .


###  http://www.sirma.com/ontologies/2016/02/culturalHeritageConservation/SMK#generalConditionAppraisalFrame
smk:generalConditionAppraisalFrame rdf:type owl:DatatypeProperty ;
                                   rdfs:subPropertyOf chc:condition ;
                                   rdfs:range xsd:string ;
                                   dc:creator "Lidiya Dimitrova"@en ;
                                   rdfs:label "General condition appraisal - frame"@en ,
                                              "Generel tilstandsvurdering ramme"@da ;
                                   skos:definition "General condition appraisal of the frame of a particular cultural object."@en .


###  http://www.sirma.com/ontologies/2016/02/culturalHeritageConservation/SMK#glazeCondition
smk:glazeCondition rdf:type owl:DatatypeProperty ;
                   rdfs:subPropertyOf chc:condition ;
                   rdfs:range xsd:string ;
                   dc:creator "Lidiya Dimitrova"@en ;
                   rdfs:label "Glaze condition"@en ,
                              "Tilstand rammeglas"@da ;
                   skos:definition "Description of the glaze condition."@en .


###  http://www.sirma.com/ontologies/2016/02/culturalHeritageConservation/SMK#glazeDescription
smk:glazeDescription rdf:type owl:DatatypeProperty ;
                     rdfs:range xsd:string ;
                     dc:creator "Lidiya Dimitrova"@en ;
                     rdfs:label "Glazing"@en ,
                                "Rammeglas"@da ;
                     skos:definition "Technical description of the glazing."@en .


###  http://www.sirma.com/ontologies/2016/02/culturalHeritageConservation/SMK#handlingNotes
smk:handlingNotes rdf:type owl:DatatypeProperty ;
                  rdfs:range xsd:string ;
                  dc:creator "Lidiya Dimitrova"@en ;
                  rdfs:label "Handling notes"@en ,
                             "Håndteringsanvisning"@da ;
                  skos:definition "Notes on preferred ways to handle a cultural object."@en .


###  http://www.sirma.com/ontologies/2016/02/culturalHeritageConservation/SMK#hasBackSideProtection
smk:hasBackSideProtection rdf:type owl:DatatypeProperty ;
                          rdfs:domain chc:CulturalObject ;
                          rdfs:range xsd:boolean ;
                          dc:creator "Lidiya Dimitrova"@en ;
                          rdfs:label "Back side protection?"@en ,
                                     "Bagklædning?"@da ;
                          skos:definition "An indication of whether the object has back side protection or not."@en .


###  http://www.sirma.com/ontologies/2016/02/culturalHeritageConservation/SMK#historicalDetailsAttached
smk:historicalDetailsAttached rdf:type owl:DatatypeProperty ;
                              rdfs:domain chc:CulturalObject ;
                              rdfs:range xsd:string ;
                              dc:creator "Lidiya Dimitrova"@en ;
                              rdfs:label "Historical details"@en ,
                                         "Historiske detaljer"@da ;
                              skos:definition "Historical details physically attached to the cultural object."@en .


###  http://www.sirma.com/ontologies/2016/02/culturalHeritageConservation/SMK#homeLocation
smk:homeLocation rdf:type owl:DatatypeProperty ;
                 rdfs:domain chc:CulturalObject ;
                 rdfs:range xsd:string ;
                 dc:creator "Lidiya Dimitrova"@en ;
                 rdfs:label "Home location"@en ,
                            "KKS/KAS placering"@da ;
                 skos:definition "The place within the organization where an object is normally located."@en .


###  http://www.sirma.com/ontologies/2016/02/culturalHeritageConservation/SMK#humidityRequirements
smk:humidityRequirements rdf:type owl:DatatypeProperty ;
                         rdfs:range xsd:string ;
                         dc:creator "Lidiya Dimitrova"@en ;
                         rdfs:label "Humidity requirements"@en ,
                                    "Krav til luftfugtighed"@da ;
                         skos:definition "Description of any special humidity requirements that the cultural object may require."@en .


###  http://www.sirma.com/ontologies/2016/02/culturalHeritageConservation/SMK#imageDimensions
smk:imageDimensions rdf:type owl:DatatypeProperty ;
                    rdfs:domain chc:CulturalObject ;
                    rdfs:range xsd:string ;
                    dc:creator "Lidiya Dimitrova"@en ;
                    rdfs:label "Billedmål"@da ,
                               "Image dimensions"@en ;
                    skos:definition "The image size of paintings, works on paper, and photographs may be smaller than the dimensions of the work."@en .


###  http://www.sirma.com/ontologies/2016/02/culturalHeritageConservation/SMK#inMicroClimateFrame
smk:inMicroClimateFrame rdf:type owl:DatatypeProperty ;
                        rdfs:domain chc:CulturalObject ;
                        rdfs:range xsd:string ;
                        dc:creator "Lidiya Dimitrova"@en ;
                        rdfs:label "Micro climate frame?"@en ,
                                   "Mikroklima ramme?"@da ;
                        skos:definition "An indication of whether the object is mounted in a micro climate frame or not."@en .


###  http://www.sirma.com/ontologies/2016/02/culturalHeritageConservation/SMK#inscriptions
smk:inscriptions rdf:type owl:DatatypeProperty ;
                 rdfs:domain chc:CulturalObject ;
                 rdfs:range xsd:string ;
                 dc:creator "Lidiya Dimitrova"@en ;
                 rdfs:label "Inscription"@en ,
                            "Påskrift"@da ;
                 skos:definition "Free text description of any writing or printing on the object's obverse or reverse. Artist signature, dealer marks, inventory codes, etc."@en .


###  http://www.sirma.com/ontologies/2016/02/culturalHeritageConservation/SMK#installationNotes
smk:installationNotes rdf:type owl:DatatypeProperty ;
                      rdfs:range xsd:string ;
                      dc:creator "Lidiya Dimitrova"@en ;
                      rdfs:label "Installation notes"@en ,
                                 "Installationsnoter"@da ;
                      skos:definition "Notes on the preferred way to install a cultural object."@en .


###  http://www.sirma.com/ontologies/2016/02/culturalHeritageConservation/SMK#installationRequirements
smk:installationRequirements rdf:type owl:DatatypeProperty ;
                             rdfs:range xsd:string ;
                             dc:creator "Lidiya Dimitrova"@en ;
                             rdfs:label "Installation requirements"@en ,
                                        "Installationskrav"@da ;
                             skos:definition "Description of requirements to borrower."@en .


###  http://www.sirma.com/ontologies/2016/02/culturalHeritageConservation/SMK#isFramed
smk:isFramed rdf:type owl:DatatypeProperty ;
             rdfs:domain chc:CulturalObject ;
             rdfs:range xsd:boolean ;
             dc:creator "Lidiya Dimitrova"@en ;
             rdfs:label "Frame?"@en ,
                        "Ramme?"@da ;
             skos:definition "Indication of whether the object is framed or not."@en .


###  http://www.sirma.com/ontologies/2016/02/culturalHeritageConservation/SMK#isLined
smk:isLined rdf:type owl:DatatypeProperty ;
            rdfs:domain chc:CulturalObject ;
            rdfs:range xsd:boolean ;
            dc:creator "Lidiya Dimitrova"@en ;
            rdfs:label "Dubleret?"@da ,
                       "Lined?"@en ;
            skos:definition "Indication of whether the object is lined or not."@en .


###  http://www.sirma.com/ontologies/2016/02/culturalHeritageConservation/SMK#legalStatus
smk:legalStatus rdf:type owl:DatatypeProperty ;
                rdfs:domain chc:CulturalObject ;
                rdfs:range xsd:string ;
                dc:creator "Lidiya Dimitrova"@en ;
                rdfs:label "Legal status"@en ,
                           "Sikkerhedsstatus"@da ;
                skos:definition "An indication of the objects legal status."@en .


###  http://www.sirma.com/ontologies/2016/02/culturalHeritageConservation/SMK#lightRequirements
smk:lightRequirements rdf:type owl:DatatypeProperty ;
                      rdfs:range xsd:string ;
                      dc:creator "Lidiya Dimitrova"@en ;
                      rdfs:label "Light requirements (lux)"@en ,
                                 "Lyskrav (lux)"@da ;
                      skos:definition "Light Requirements (lux) for the cultural object."@en .


###  http://www.sirma.com/ontologies/2016/02/culturalHeritageConservation/SMK#marks
smk:marks rdf:type owl:DatatypeProperty ;
          rdfs:domain chc:CulturalObject ;
          rdfs:range xsd:string ;
          dc:creator "Lidiya Dimitrova"@en ;
          rdfs:label "Marks"@en ,
                     "Mærker"@da ;
          skos:definition "Description of any marks not related to the image such notations or marks made by a processes."@en .


###  http://www.sirma.com/ontologies/2016/02/culturalHeritageConservation/SMK#materials
smk:materials rdf:type owl:DatatypeProperty ;
              rdfs:domain chc:CulturalObject ;
              rdfs:range xsd:string ;
              dc:creator "Lidiya Dimitrova"@en ;
              rdfs:label "Material"@en ,
                         "Materiale"@da ;
              skos:definition "The basic materials and media from which an object is constructed."@en .


###  http://www.sirma.com/ontologies/2016/02/culturalHeritageConservation/SMK#mediaCondition
smk:mediaCondition rdf:type owl:DatatypeProperty ;
                   rdfs:subPropertyOf chc:condition ;
                   rdfs:range xsd:string ;
                   dc:creator "Lidiya Dimitrova"@en ;
                   rdfs:label "Media condition"@en ,
                              "Tilstand medie"@da ;
                   skos:definition "General description of condition of the media used in a drawing."@en .


###  http://www.sirma.com/ontologies/2016/02/culturalHeritageConservation/SMK#medium
smk:medium rdf:type owl:DatatypeProperty ;
           rdfs:domain chc:CulturalObject ;
           rdfs:range xsd:string ;
           dc:creator "Lidiya Dimitrova"@en ;
           rdfs:label "Medium"@da ,
                      "Medium"@en ;
           skos:definition "Medium description often used for public."@en .


###  http://www.sirma.com/ontologies/2016/02/culturalHeritageConservation/SMK#mountCondition
smk:mountCondition rdf:type owl:DatatypeProperty ;
                   rdfs:subPropertyOf chc:condition ;
                   rdfs:domain chc:CulturalObject ;
                   rdfs:range xsd:string ;
                   dc:creator "Lidiya Dimitrova"@en ;
                   rdfs:label "Montering tilstand"@da ,
                              "Mount condition"@en ;
                   skos:definition "Description of the mount condition."@en .


###  http://www.sirma.com/ontologies/2016/02/culturalHeritageConservation/SMK#mountDescription
smk:mountDescription rdf:type owl:DatatypeProperty ;
                     rdfs:range xsd:string ;
                     dc:creator "Lidiya Dimitrova"@en ;
                     rdfs:label "Montering"@da ,
                                "Mount"@en ;
                     skos:definition "Technical description of the mount."@en .


###  http://www.sirma.com/ontologies/2016/02/culturalHeritageConservation/SMK#objectStatus
smk:objectStatus rdf:type owl:DatatypeProperty ;
                 rdfs:domain chc:CulturalObject ;
                 rdfs:range xsd:string ;
                 dc:creator "Lidiya Dimitrova"@en ;
                 rdfs:label "Object status"@en ,
                            "Værkstatus"@da ;
                 skos:definition "A statement of the standing of an object in relation to others in existence."@en .


###  http://www.sirma.com/ontologies/2016/02/culturalHeritageConservation/SMK#orientation
smk:orientation rdf:type owl:DatatypeProperty ;
                rdfs:range xsd:string ;
                dc:creator "Lidiya Dimitrova"@en ;
                rdfs:label "Orientation"@en ,
                           "Retning/orientering"@da ;
                skos:definition "Orientation of the art object."@en .


###  http://www.sirma.com/ontologies/2016/02/culturalHeritageConservation/SMK#ownerName
smk:ownerName rdf:type owl:DatatypeProperty ;
              rdfs:domain chc:CulturalObject ;
              rdfs:range xsd:string ;
              dc:creator "Lidiya Dimitrova"@en ;
              rdfs:label "Ejerens navn"@da ,
                         "Owner name"@en ;
              skos:definition "The owner (person or organization) of an object if not in the museum's possession."@en .


###  http://www.sirma.com/ontologies/2016/02/culturalHeritageConservation/SMK#packingNotes
smk:packingNotes rdf:type owl:DatatypeProperty ;
                 rdfs:range xsd:string ;
                 dc:creator "Lidiya Dimitrova"@en ;
                 rdfs:label "Packing notes"@en ,
                            "Pakningsanvisning"@da ;
                 skos:definition "Notes on how a cultural object should best be packed for movement or transport."@en .


###  http://www.sirma.com/ontologies/2016/02/culturalHeritageConservation/SMK#paintLayersCondition
smk:paintLayersCondition rdf:type owl:DatatypeProperty ;
                         rdfs:subPropertyOf chc:condition ;
                         rdfs:range xsd:string ;
                         dc:creator "Lidiya Dimitrova"@en ;
                         rdfs:label "Paint layers condition"@en ,
                                    "Tilstand farvelag"@da ;
                         skos:definition "Technical description of condition of the paint layers."@en .


###  http://www.sirma.com/ontologies/2016/02/culturalHeritageConservation/SMK#paintLayersDescription
smk:paintLayersDescription rdf:type owl:DatatypeProperty ;
                           rdfs:domain chc:CulturalObject ;
                           rdfs:range xsd:string ;
                           dc:creator "Lidiya Dimitrova"@en ;
                           rdfs:label "Farvelag"@da ,
                                      "Paint layers"@en ;
                           skos:definition "Technical description of the paint layer or design construction."@en .


###  http://www.sirma.com/ontologies/2016/02/culturalHeritageConservation/SMK#portfolioTitle
smk:portfolioTitle rdf:type owl:DatatypeProperty ;
                   rdfs:domain chc:CulturalObject ;
                   rdfs:range xsd:string ;
                   dc:creator "Lidiya Dimitrova"@en ;
                   rdfs:label "Portfolio/Serie"@da ,
                              "Portfolio/Series"@en ;
                   skos:definition "Indication of a group of works of art created as a group."@en .


###  http://www.sirma.com/ontologies/2016/02/culturalHeritageConservation/SMK#primingCondition
smk:primingCondition rdf:type owl:DatatypeProperty ;
                     rdfs:subPropertyOf chc:condition ;
                     rdfs:range xsd:string ;
                     dc:creator "Lidiya Dimitrova"@en ;
                     rdfs:label "Sizing and ground condition"@en ,
                                "Tilstand forlimning og grundering"@da ;
                     skos:definition "A technical description of the stretcher/strainer condition."@en .


###  http://www.sirma.com/ontologies/2016/02/culturalHeritageConservation/SMK#primingDescription
smk:primingDescription rdf:type owl:DatatypeProperty ;
                       rdfs:domain chc:CulturalObject ;
                       rdfs:range xsd:string ;
                       dc:creator "Lidiya Dimitrova"@en ;
                       rdfs:label "Forlimning og grundering"@da ,
                                  "Sizing and ground"@en ;
                       skos:definition "Technical description of the sizing and ground construction."@en .


###  http://www.sirma.com/ontologies/2016/02/culturalHeritageConservation/SMK#provenance
smk:provenance rdf:type owl:DatatypeProperty ;
               rdfs:domain chc:CulturalObject ;
               rdfs:range xsd:string ;
               dc:creator "Lidiya Dimitrova"@en ;
               rdfs:label "Provenance"@en ,
                          "Proveniens"@da ;
               skos:definition "Description of the historical ownership of the object."@en .


###  http://www.sirma.com/ontologies/2016/02/culturalHeritageConservation/SMK#recordingAnalogueMediaType
smk:recordingAnalogueMediaType rdf:type owl:DatatypeProperty ;
                               rdfs:range xsd:string ;
                               dc:creator "Lidiya Dimitrova"@en ;
                               rdfs:label "Media type (analogue)"@en ,
                                          "Medietype (analog)"@da ;
                               skos:definition "Description of the file format of the Media type (analogue)."@en .


###  http://www.sirma.com/ontologies/2016/02/culturalHeritageConservation/SMK#recordingColour
smk:recordingColour rdf:type owl:DatatypeProperty ;
                    rdfs:range xsd:string ;
                    dc:creator "Lidiya Dimitrova"@en ;
                    rdfs:label "Colour"@en ,
                               "Farve"@da ;
                    skos:definition "Indication of whether the recording is in b/w or colour."@en .


###  http://www.sirma.com/ontologies/2016/02/culturalHeritageConservation/SMK#recordingDate
smk:recordingDate rdf:type owl:DatatypeProperty ;
                  rdfs:range xsd:string ;
                  dc:creator "Lidiya Dimitrova"@en ;
                  rdfs:label "Date of recording"@en ,
                             "Dato for optagelse"@da ;
                  skos:definition "Information on the date when the recording was made."@en .


###  http://www.sirma.com/ontologies/2016/02/culturalHeritageConservation/SMK#recordingDigitalMediaType
smk:recordingDigitalMediaType rdf:type owl:DatatypeProperty ;
                              rdfs:range xsd:string ;
                              dc:creator "Lidiya Dimitrova"@en ;
                              rdfs:label "Media type (digital)"@en ,
                                         "Medietype (digital)"@da ;
                              skos:definition "Description of the file format of the Media type (digital)."@en .


###  http://www.sirma.com/ontologies/2016/02/culturalHeritageConservation/SMK#recordingFormat
smk:recordingFormat rdf:type owl:DatatypeProperty ;
                    rdfs:range xsd:string ;
                    dc:creator "Lidiya Dimitrova"@en ;
                    rdfs:label "Format"@da ,
                               "Format"@en ;
                    skos:definition "Indication of the format of the recording."@en .


###  http://www.sirma.com/ontologies/2016/02/culturalHeritageConservation/SMK#recordingFramerate
smk:recordingFramerate rdf:type owl:DatatypeProperty ;
                       rdfs:range xsd:string ;
                       dc:creator "Lidiya Dimitrova"@en ;
                       rdfs:label "Billedfrekvens"@da ,
                                  "Framerate"@en ;
                       skos:definition "Description of the framerate of the recording."@en .


###  http://www.sirma.com/ontologies/2016/02/culturalHeritageConservation/SMK#recordingLabel
smk:recordingLabel rdf:type owl:DatatypeProperty ;
                   rdfs:range xsd:string ;
                   dc:creator "Lidiya Dimitrova"@en ;
                   rdfs:label "Label for artist's master and exhibition copy"@en ,
                              "Label for kunstners master- og udstillingskopi"@da ;
                   skos:definition "Indication of the nature of the label."@en .


###  http://www.sirma.com/ontologies/2016/02/culturalHeritageConservation/SMK#recordingPictureQuality
smk:recordingPictureQuality rdf:type owl:DatatypeProperty ;
                            rdfs:range xsd:string ;
                            dc:creator "Lidiya Dimitrova"@en ;
                            rdfs:label "Billedkvalitet"@da ,
                                       "Picture quality"@en ;
                            skos:definition "A description of the picture quality of the reording"@en .


###  http://www.sirma.com/ontologies/2016/02/culturalHeritageConservation/SMK#recordingResolution
smk:recordingResolution rdf:type owl:DatatypeProperty ;
                        rdfs:range xsd:string ;
                        dc:creator "Lidiya Dimitrova"@en ;
                        rdfs:label "Løsning/afklaring"@da ,
                                   "Resolution"@en ;
                        skos:definition "Description of the resolution of the recording."@en .


###  http://www.sirma.com/ontologies/2016/02/culturalHeritageConservation/SMK#recordingSound
smk:recordingSound rdf:type owl:DatatypeProperty ;
                   rdfs:range xsd:string ;
                   dc:creator "Lidiya Dimitrova"@en ;
                   rdfs:label "Lyd"@da ,
                              "Sound"@en ;
                   skos:definition "Indication of characteristics of the sound of the recording."@en .


###  http://www.sirma.com/ontologies/2016/02/culturalHeritageConservation/SMK#recordingSoundQuality
smk:recordingSoundQuality rdf:type owl:DatatypeProperty ;
                          rdfs:range xsd:string ;
                          dc:creator "Lidiya Dimitrova"@en ;
                          rdfs:label "Lydkvalitet"@da ,
                                     "Sound quality"@en ;
                          skos:definition "A description of the sound quality of the recording."@en .


###  http://www.sirma.com/ontologies/2016/02/culturalHeritageConservation/SMK#recordingSpokenLanguage
smk:recordingSpokenLanguage rdf:type owl:DatatypeProperty ;
                            rdfs:range xsd:string ;
                            dc:creator "Lidiya Dimitrova"@en ;
                            rdfs:label "Spoken language"@en ,
                                       "Talesprog"@da ;
                            skos:definition "Language spoken on the recording."@en .


###  http://www.sirma.com/ontologies/2016/02/culturalHeritageConservation/SMK#recordingStandard
smk:recordingStandard rdf:type owl:DatatypeProperty ;
                      rdfs:range xsd:string ;
                      dc:creator "Lidiya Dimitrova"@en ;
                      rdfs:label "TV standard"@en ,
                                 "TV-standard"@da ;
                      skos:definition "List for indication of TV standard to which the recording is complied"@en .


###  http://www.sirma.com/ontologies/2016/02/culturalHeritageConservation/SMK#recordingStudio
smk:recordingStudio rdf:type owl:DatatypeProperty ;
                    rdfs:range xsd:string ;
                    dc:creator "Lidiya Dimitrova"@en ;
                    rdfs:label "A/V studie"@da ,
                               "A/V studio"@en ;
                    skos:definition "The name of the A/V studio that did the recording."@en .


###  http://www.sirma.com/ontologies/2016/02/culturalHeritageConservation/SMK#recordingSubtitles
smk:recordingSubtitles rdf:type owl:DatatypeProperty ;
                       rdfs:range xsd:string ;
                       dc:creator "Lidiya Dimitrova"@en ;
                       rdfs:label "Subtitles"@en ,
                                  "Undertitler"@da ;
                       skos:definition "Description of the subtitles in the recording."@en .


###  http://www.sirma.com/ontologies/2016/02/culturalHeritageConservation/SMK#recordingVideoType
smk:recordingVideoType rdf:type owl:DatatypeProperty ;
                       rdfs:range xsd:string ;
                       dc:creator "Lidiya Dimitrova"@en ;
                       rdfs:label "Video type"@en ,
                                  "Videotype"@da ;
                       skos:definition "Description of the video type."@en .


###  http://www.sirma.com/ontologies/2016/02/culturalHeritageConservation/SMK#recordingViewedDescription
smk:recordingViewedDescription rdf:type owl:DatatypeProperty ;
                               rdfs:range xsd:string ;
                               dc:creator "Lidiya Dimitrova"@en ;
                               rdfs:label "Set"@da ,
                                          "Viewed"@en ;
                               skos:definition "A description of when and and under what circumstances the recording was viewed."@en .


###  http://www.sirma.com/ontologies/2016/02/culturalHeritageConservation/SMK#sampleCondition
smk:sampleCondition rdf:type owl:DatatypeProperty ;
                    rdfs:subPropertyOf chc:condition ;
                    rdfs:range xsd:string ;
                    dc:creator "Lidiya Dimitrova"@en ;
                    rdfs:label "Sample condition"@en ,
                               "Tilstand materialeprøve"@da ;
                    skos:definition "Materials identified in the analysis of the sample: \"chrome yellow in linseed oil."@en .


###  http://www.sirma.com/ontologies/2016/02/culturalHeritageConservation/SMK#sampleMaterialsIdentified
smk:sampleMaterialsIdentified rdf:type owl:DatatypeProperty ;
                              rdfs:range xsd:string ;
                              dc:creator "Lidiya Dimitrova"@en ;
                              rdfs:label "Identificerede materialer"@da ,
                                         "Materials identified"@en ;
                              skos:definition "Materials identified in the analysis of the sample: \"chrome yellow in linseed oil."@en .


###  http://www.sirma.com/ontologies/2016/02/culturalHeritageConservation/SMK#samplePhysicalLocation
smk:samplePhysicalLocation rdf:type owl:DatatypeProperty ;
                           rdfs:range xsd:string ;
                           dc:creator "Lidiya Dimitrova"@en ;
                           rdfs:label "Fysisk placering"@da ,
                                      "Physical location"@en ;
                           skos:definition "Physical location of the sample so that someone could lay their hands on such as drawer number."@en .


###  http://www.sirma.com/ontologies/2016/02/culturalHeritageConservation/SMK#sampleSite
smk:sampleSite rdf:type owl:DatatypeProperty ;
               rdfs:range xsd:string ;
               dc:creator "Lidiya Dimitrova"@en ;
               rdfs:label "Lokalitet materialeprøve"@da ,
                          "Sample site"@en ;
               skos:definition "Location of the spot where the sample was taken: coordinates \"up\" and \"left\" or \"from right hand of the sitter\"."@en .


###  http://www.sirma.com/ontologies/2016/02/culturalHeritageConservation/SMK#samplingDate
smk:samplingDate rdf:type owl:DatatypeProperty ;
                 rdfs:range xsd:dateTime ;
                 dc:creator "Lidiya Dimitrova"@en ;
                 rdfs:label "Date taken"@en ,
                            "Dato for udtagelse"@da ;
                 skos:definition "Date on which the sample was taken."@en .


###  http://www.sirma.com/ontologies/2016/02/culturalHeritageConservation/SMK#secondarySupportDistinguishingMarks
smk:secondarySupportDistinguishingMarks rdf:type owl:DatatypeProperty ;
                                        rdfs:range xsd:string ;
                                        dc:creator "Lidiya Dimitrova"@en ;
                                        rdfs:label "Auxiliary support distinguishing marks"@en ,
                                                   "Kendetegn bærende underlag"@da ;
                                        skos:definition "Marks on the secondary support that may help to distinguish this cultural object from a different version"@en .


###  http://www.sirma.com/ontologies/2016/02/culturalHeritageConservation/SMK#stretcher
smk:stretcher rdf:type owl:DatatypeProperty ;
              rdfs:range xsd:string ;
              dc:creator "Lidiya Dimitrova"@en ;
              rdfs:label "Kileramme/fast spændramme"@da ,
                         "Stretcher/strainer"@en ;
              skos:definition "Technical description of the stretcher/strainer."@en .


###  http://www.sirma.com/ontologies/2016/02/culturalHeritageConservation/SMK#stretcherCondition
smk:stretcherCondition rdf:type owl:DatatypeProperty ;
                       rdfs:subPropertyOf chc:condition ;
                       rdfs:range xsd:string ;
                       dc:creator "Lidiya Dimitrova"@en ;
                       rdfs:label "Stretcher/strainer condition"@en ,
                                  "Tilstand kileramme/fast spændramme"@da ;
                       skos:definition "Description of the stretcher/strainer condition."@en .


###  http://www.sirma.com/ontologies/2016/02/culturalHeritageConservation/SMK#stretcherDistinguishingMarks
smk:stretcherDistinguishingMarks rdf:type owl:DatatypeProperty ;
                                 rdfs:range xsd:string ;
                                 dc:creator "Lidiya Dimitrova"@en ;
                                 rdfs:label "Kendetegn kileramme/fast spændramme"@da ,
                                            "Stretcher/strainer distinguishing marks"@en ;
                                 skos:definition "Marks on the stretcher/strainer that may help to distinguish it."@en .


###  http://www.sirma.com/ontologies/2016/02/culturalHeritageConservation/SMK#structureCondition
smk:structureCondition rdf:type owl:DatatypeProperty ;
                       rdfs:subPropertyOf chc:condition ;
                       rdfs:range xsd:string ;
                       dc:creator "Lidiya Dimitrova"@en ;
                       rdfs:label "Structural condition"@en ,
                                  "Tilstand strukturelt"@da ;
                       skos:definition "Description of structural condition of a cultural object."@en .


###  http://www.sirma.com/ontologies/2016/02/culturalHeritageConservation/SMK#subType
smk:subType rdf:type owl:DatatypeProperty ;
            rdfs:range xsd:string ;
            dc:creator "Lidiya Dimitrova"@en ;
            rdfs:label "Object sub-type"@en ,
                       "Undertype"@en ;
            skos:definition "Sub-Classification of the object."@en .


###  http://www.sirma.com/ontologies/2016/02/culturalHeritageConservation/SMK#supportCondition
smk:supportCondition rdf:type owl:DatatypeProperty ;
                     rdfs:subPropertyOf chc:condition ;
                     rdfs:range xsd:string ;
                     dc:creator "Lidiya Dimitrova"@en ;
                     rdfs:label "Support condition"@en ,
                                "Tilstand bærende underlag"@da ;
                     skos:definition "Description of the support condition of the cultural object."@en .


###  http://www.sirma.com/ontologies/2016/02/culturalHeritageConservation/SMK#supportDescription
smk:supportDescription rdf:type owl:DatatypeProperty ;
                       rdfs:domain chc:CulturalObject ;
                       rdfs:range xsd:string ;
                       dc:creator "Lidiya Dimitrova"@en ;
                       rdfs:label "Bærende underlag"@da ,
                                  "Support"@en ;
                       skos:definition "Technical description of the support, in case of painting on canvas - the description of canvas."@en .


###  http://www.sirma.com/ontologies/2016/02/culturalHeritageConservation/SMK#supportDistinguishingMarks
smk:supportDistinguishingMarks rdf:type owl:DatatypeProperty ;
                               rdfs:domain chc:CulturalObject ;
                               rdfs:range xsd:string ;
                               dc:creator "Lidiya Dimitrova"@en ;
                               rdfs:label "Kendetegn bærende underlag"@da ,
                                          "Support distinguishing marks"@en ;
                               skos:definition "Description of any marks not related to the image such notations or marks on the support."@en .


###  http://www.sirma.com/ontologies/2016/02/culturalHeritageConservation/SMK#supportType
smk:supportType rdf:type owl:DatatypeProperty ;
                rdfs:range xsd:string ;
                dc:creator "Lidiya Dimitrova"@en ;
                rdfs:label "Support type"@en ,
                           "Type bærende underlag"@da ;
                skos:definition "Description of the type of the support of the cultural object."@en .


###  http://www.sirma.com/ontologies/2016/02/culturalHeritageConservation/SMK#surfaceCoating
smk:surfaceCoating rdf:type owl:DatatypeProperty ;
                   rdfs:domain chc:CulturalObject ;
                   rdfs:range xsd:boolean ;
                   dc:creator "Lidiya Dimitrova"@en ;
                   rdfs:label "Overfladebehandling (ja/nej)"@da ,
                              "Surface coating (Yes, or No)"@en ;
                   skos:definition "Yes or No, whether a final varnish has been applied to the painting."@en .


###  http://www.sirma.com/ontologies/2016/02/culturalHeritageConservation/SMK#surfaceCoatingCondition
smk:surfaceCoatingCondition rdf:type owl:DatatypeProperty ;
                            rdfs:subPropertyOf chc:condition ;
                            rdfs:range xsd:string ;
                            dc:creator "Lidiya Dimitrova"@en ;
                            rdfs:label "Surface coating condition"@en ,
                                       "Tilstand overfladebehandling"@da ;
                            skos:definition "Technical description of the condition of the surface coating."@en .


###  http://www.sirma.com/ontologies/2016/02/culturalHeritageConservation/SMK#surfaceCoatingMaterial
smk:surfaceCoatingMaterial rdf:type owl:DatatypeProperty ;
                           rdfs:domain chc:CulturalObject ;
                           rdfs:range xsd:string ;
                           dc:creator "Lidiya Dimitrova"@en ;
                           rdfs:label "Materiale overfladebehandling"@da ,
                                      "Surface coating material"@en ;
                           skos:definition "Technical description of the surface coating material."@en .


###  http://www.sirma.com/ontologies/2016/02/culturalHeritageConservation/SMK#surfaceCondition
smk:surfaceCondition rdf:type owl:DatatypeProperty ;
                     rdfs:subPropertyOf chc:condition ;
                     rdfs:range xsd:string ;
                     dc:creator "Lidiya Dimitrova"@en ;
                     rdfs:label "Surface condition"@en ,
                                "Tilstand overflade"@da ;
                     skos:definition "Description of surface condition of a cultural object."@en .


###  http://www.sirma.com/ontologies/2016/02/culturalHeritageConservation/SMK#technique
smk:technique rdf:type owl:DatatypeProperty ;
              rdfs:range xsd:string ;
              dc:creator "Lidiya Dimitrova"@en ;
              rdfs:label "Technique"@en ,
                         "Teknik"@da ;
              skos:definition "Description on how the cultural object is made."@en .


###  http://www.sirma.com/ontologies/2016/02/culturalHeritageConservation/SMK#temperatureRequirements
smk:temperatureRequirements rdf:type owl:DatatypeProperty ;
                            rdfs:range xsd:string ;
                            dc:creator "Lidiya Dimitrova"@en ;
                            rdfs:label "Temperature requirements"@en ,
                                       "Temperaturkrav"@da ;
                            skos:definition "Temperature requirements for the cultural object."@en .


###  http://www.sirma.com/ontologies/2016/02/culturalHeritageConservation/SMK#titleAlternative
smk:titleAlternative rdf:type owl:DatatypeProperty ;
                     rdfs:domain chc:CulturalObject ;
                     rdfs:range xsd:string ;
                     dc:creator "Lidiya Dimitrova"@en ;
                     rdfs:label "Anden titel"@da ,
                                "Title (alternative)"@en ;
                     skos:definition "Temporary primary title for use strictly in the context of an exhibition or publication. May be more than one."@en .


###  http://www.sirma.com/ontologies/2016/02/culturalHeritageConservation/SMK#transportNotes
smk:transportNotes rdf:type owl:DatatypeProperty ;
                   rdfs:range xsd:string ;
                   dc:creator "Lidiya Dimitrova"@en ;
                   rdfs:label "Transport notes"@en ,
                              "Transportanvisning"@da ;
                   skos:definition "Notes on the preferred way to transport a cultural object."@en .


###  http://www.sirma.com/ontologies/2016/02/culturalHeritageConservation/SMK#treatmentType
smk:treatmentType rdf:type owl:DatatypeProperty ;
                  rdfs:range xsd:string ;
                  dc:creator "Malvina Makarieva"@en ;
                  rdfs:label "Behandling"@da ,
                             "Treatment"@en ;
                  skos:definition "Indicates if the treatment is minor or major."@en .


###  http://www.sirma.com/ontologies/2016/02/culturalHeritageConservation/SMK#weight
smk:weight rdf:type owl:DatatypeProperty ;
           rdfs:domain chc:CulturalObject ;
           rdfs:range xsd:string ;
           dc:creator "Lidiya Dimitrova"@en ;
           rdfs:label "Vægt"@da ,
                      "Weight"@en ;
           skos:definition "The weight of an object"@en .


#################################################################
#    Classes
#################################################################

###  http://www.sirma.com/ontologies/2016/02/culturalHeritageConservation#CulturalObject
chc:CulturalObject emf:isSearchable "true"^^xsd:boolean .


###  http://www.sirma.com/ontologies/2016/02/culturalHeritageConservation/SMK#Cast
smk:Cast rdf:type owl:Class ;
         rdfs:subClassOf chc:CulturalObject ;
         emf:classCategory "culturalobject" ;
         emf:definitionId "objectinstance" ;
         emf:isCreateable "true"^^xsd:boolean ;
         emf:isPartOfObjectLibrary "true"^^xsd:boolean ;
         emf:isSearchable "true"^^xsd:boolean ;
         dc:creator "Lidiya Dimitrova"@en ;
         sec:allowInheritLibraryPermissions "true"^^xsd:boolean ;
         sec:allowInheritParentPermissions "false"^^xsd:boolean ;
         rdfs:label "Afstøbning"@da ,
                    "Cast"@en ;
         skos:definition "In art a plaster cast is a copy made in plaster of another 3-dimensional form. The original from which the cast is taken may be a sculpture, or a fragment of a building. Typically cast collections were created as study collections containing copies of masterworks from Western antiquity, medieval, and renaissance art."@en .


###  http://www.sirma.com/ontologies/2016/02/culturalHeritageConservation/SMK#Collage
smk:Collage rdf:type owl:Class ;
            rdfs:subClassOf chc:CulturalObject ;
            emf:classCategory "culturalobject" ;
            emf:definitionId "objectinstance" ;
            emf:isCreateable "true"^^xsd:boolean ;
            emf:isPartOfObjectLibrary "true"^^xsd:boolean ;
            emf:isSearchable "true"^^xsd:boolean ;
            dc:creator "Malvina Makarieva"@en ;
            sec:allowInheritLibraryPermissions "true"^^xsd:boolean ;
            sec:allowInheritParentPermissions "false"^^xsd:boolean ;
            rdfs:label "Collage"@da ,
                       "Collage"@en ;
            skos:definition "Collage is a technique of an art production, primarily used in the visual arts, where the artwork is made from an assemblage of different forms, thus creating a new whole. A collage may sometimes include magazine and newspaper clippings, ribbons, paint, bits of colored or handmade papers, portions of other artwork or texts, photographs and other found objects, glued to a piece of paper or canvas. The origins of collage can be traced back hundreds of years, but this technique made a dramatic reappearance in the early 20th century as an art form of novelty. The term collage was coined by both Georges Braque and Pablo Picasso in the beginning of the 20th century when collage became a distinctive part of modern art. (Wikipedia)."@en .


###  http://www.sirma.com/ontologies/2016/02/culturalHeritageConservation/SMK#DecorativeArt
smk:DecorativeArt rdf:type owl:Class ;
                  rdfs:subClassOf chc:CulturalObject ;
                  emf:classCategory "culturalobject" ;
                  emf:definitionId "objectinstance" ;
                  emf:isCreateable "true"^^xsd:boolean ;
                  emf:isPartOfObjectLibrary "true"^^xsd:boolean ;
                  emf:isSearchable "true"^^xsd:boolean ;
                  dc:creator "Lidiya Dimitrova"@en ;
                  sec:allowInheritLibraryPermissions "true"^^xsd:boolean ;
                  sec:allowInheritParentPermissions "false"^^xsd:boolean ;
                  rdfs:label "Decorative Art"@en ,
                             "Kunsthåndværk"@da ;
                  skos:definition "The decorative arts are arts or crafts concerned with the design and manufacture of beautiful objects that are also functional. It includes interior design, but not usually architecture . Examples include things like candle sticks, furniture, porcelain dinnerware, etc."@en .


###  http://www.sirma.com/ontologies/2016/02/culturalHeritageConservation/SMK#Drawing
smk:Drawing rdf:type owl:Class ;
            rdfs:subClassOf chc:CulturalObject ;
            emf:classCategory "culturalobject" ;
            emf:definitionId "objectinstance" ;
            emf:isCreateable "true"^^xsd:boolean ;
            emf:isPartOfObjectLibrary "true"^^xsd:boolean ;
            emf:isSearchable "true"^^xsd:boolean ;
            dc:creator "Kiril Penev"@en ;
            sec:allowInheritLibraryPermissions "true"^^xsd:boolean ;
            sec:allowInheritParentPermissions "false"^^xsd:boolean ;
            rdfs:label "Drawing"@en ,
                       "Tegning"@da ;
            skos:definition "Drawing is a form of visual art that makes use of any number of drawing instruments to mark a two-dimensional medium. Instruments used include graphite pencils, pen and ink, inked brushes, wax color pencils, crayons, charcoal, chalk, pastels, various kinds of erasers, markers, styluses, and various metals (such as silverpoint) (Wikipedia)."@en .


###  http://www.sirma.com/ontologies/2016/02/culturalHeritageConservation/SMK#Frame
smk:Frame rdf:type owl:Class ;
          rdfs:subClassOf chc:CulturalObject ;
          emf:classCategory "culturalobject" ;
          emf:definitionId "objectinstance" ;
          emf:isCreateable "true"^^xsd:boolean ;
          emf:isPartOfObjectLibrary "true"^^xsd:boolean ;
          emf:isSearchable "true"^^xsd:boolean ;
          dc:creator "Lidiya Dimitrova"@en ;
          sec:allowInheritLibraryPermissions "true"^^xsd:boolean ;
          sec:allowInheritParentPermissions "false"^^xsd:boolean ;
          rdfs:label "Frame"@en ,
                     "Ramme"@da ;
          skos:definition "A frame is a decorative molding that typically is attached to a painting or other cultural object especially when that cultural object is displayed. It typically surrounds and covers the edges of the cultural object. It is typically made of wood/plaster/gold leaf, but can be any material."@en .


###  http://www.sirma.com/ontologies/2016/02/culturalHeritageConservation/SMK#Installation
smk:Installation rdf:type owl:Class ;
                 rdfs:subClassOf chc:CulturalObject ;
                 emf:classCategory "culturalobject" ;
                 emf:definitionId "objectinstance" ;
                 emf:isCreateable "true"^^xsd:boolean ;
                 emf:isPartOfObjectLibrary "true"^^xsd:boolean ;
                 emf:isSearchable "true"^^xsd:boolean ;
                 dc:creator "Lidiya Dimitrova"@en ;
                 sec:allowInheritLibraryPermissions "true"^^xsd:boolean ;
                 sec:allowInheritParentPermissions "false"^^xsd:boolean ;
                 rdfs:label "Installation"@da ,
                            "Installation"@en ;
                 skos:definition "Installation art is an artistic genre of three-dimensional works that often are site-specific and designed to transform the perception of a space. Generally, the term is applied to interior spaces, whereas exterior interventions are often called public art, land art or intervention art; however, the boundaries between these terms overlap. (Wikipedia)."@en .


###  http://www.sirma.com/ontologies/2016/02/culturalHeritageConservation/SMK#MediaArt
smk:MediaArt rdf:type owl:Class ;
             rdfs:subClassOf chc:CulturalObject ;
             emf:classCategory "culturalobject" ;
             emf:definitionId "objectinstance" ;
             emf:isCreateable "true"^^xsd:boolean ;
             emf:isPartOfObjectLibrary "true"^^xsd:boolean ;
             emf:isSearchable "true"^^xsd:boolean ;
             dc:creator "Lidiya Dimitrova"@en ;
             sec:allowInheritLibraryPermissions "true"^^xsd:boolean ;
             sec:allowInheritParentPermissions "false"^^xsd:boolean ;
             rdfs:label "Audiovisuel kunst"@da ,
                        "Media Art"@en ;
             skos:definition "Media art is a genre that encompasses artworks created with new media technologies, including digital art, computer animation, computer graphics, virtual art, internet art, interactive art, video games, computer robotics, 3-D printing, and art as biotechnology. It can also include film if not represented elsewhere."@en .


###  http://www.sirma.com/ontologies/2016/02/culturalHeritageConservation/SMK#Painting
smk:Painting rdf:type owl:Class ;
             rdfs:subClassOf chc:CulturalObject ;
             emf:classCategory "culturalobject" ;
             emf:definitionId "objectinstance" ;
             emf:isCreateable "true"^^xsd:boolean ;
             emf:isPartOfObjectLibrary "true"^^xsd:boolean ;
             emf:isSearchable "true"^^xsd:boolean ;
             dc:creator "Kiril Penev"@en ;
             sec:allowInheritLibraryPermissions "true"^^xsd:boolean ;
             sec:allowInheritParentPermissions "false"^^xsd:boolean ;
             rdfs:label "Maleri"@da ,
                        "Painting"@en ;
             skos:definition "Painting is the practice of applying paint, pigment, color or other medium to a surface (support base). The medium is commonly applied to the base with a brush but other implements, such as knives, sponges, and airbrushes, can be used. In art, the term painting describes both the act and the result of the action. However, painting is also used outside of art as a common trade among craftsmen and builders. Paintings may have for their support such surfaces as walls, paper, canvas, wood, glass, lacquer, clay, leaf, copper or concrete, and may incorporate multiple other materials including sand, clay, paper, gold leaf as well as objects (Wikipedia)."@en .


###  http://www.sirma.com/ontologies/2016/02/culturalHeritageConservation/SMK#Photograph
smk:Photograph rdf:type owl:Class ;
               rdfs:subClassOf chc:CulturalObject ;
               emf:classCategory "culturalobject" ;
               emf:definitionId "objectinstance" ;
               emf:isCreateable "true"^^xsd:boolean ;
               emf:isPartOfObjectLibrary "true"^^xsd:boolean ;
               emf:isSearchable "true"^^xsd:boolean ;
               dc:creator "Kiril Penev"@en ;
               sec:allowInheritLibraryPermissions "true"^^xsd:boolean ;
               sec:allowInheritParentPermissions "false"^^xsd:boolean ;
               rdfs:label "Fotografi"@da ,
                          "Photograph"@en ;
               skos:definition "A photograph or photo is an image created by light falling on a light-sensitive surface, usually photographic film or an electronic image such as a CCD or a CMOS chip. Most photographs are created using a camera, which uses a lens to focus the scene's visible wavelengths of light into a reproduction of what the human eye would see. (Wikipedia)."@en .


###  http://www.sirma.com/ontologies/2016/02/culturalHeritageConservation/SMK#Print
smk:Print rdf:type owl:Class ;
          rdfs:subClassOf chc:CulturalObject ;
          emf:classCategory "culturalobject" ;
          emf:definitionId "objectinstance" ;
          emf:isCreateable "true"^^xsd:boolean ;
          emf:isPartOfObjectLibrary "true"^^xsd:boolean ;
          emf:isSearchable "true"^^xsd:boolean ;
          dc:creator "Kiril Penev"@en ;
          sec:allowInheritLibraryPermissions "true"^^xsd:boolean ;
          sec:allowInheritParentPermissions "false"^^xsd:boolean ;
          rdfs:label "Grafik"@da ,
                     "Print"@en ;
          skos:definition """A picture or design printed from a block or plate or copied from a painting by photography.
A piece of fabric or clothing with a decorative colored pattern or design printed on it."""@en .


###  http://www.sirma.com/ontologies/2016/02/culturalHeritageConservation/SMK#Sculpture
smk:Sculpture rdf:type owl:Class ;
              rdfs:subClassOf chc:CulturalObject ;
              emf:classCategory "culturalobject" ;
              emf:definitionId "objectinstance" ;
              emf:isCreateable "true"^^xsd:boolean ;
              emf:isPartOfObjectLibrary "true"^^xsd:boolean ;
              emf:isSearchable "true"^^xsd:boolean ;
              dc:creator "Kiril Penev"@en ;
              sec:allowInheritLibraryPermissions "true"^^xsd:boolean ;
              sec:allowInheritParentPermissions "false"^^xsd:boolean ;
              rdfs:label "Sculpture"@en ,
                         "Skulptur"@da ;
              skos:definition "Sculpture is the branch of the visual arts that operates in three dimensions, and one of the plastic arts. Durable sculptural processes originally used carving (the removal of material) and modelling (the addition of material, as clay), in stone, metal, ceramics, wood and other materials but, since modernism, shifts in sculptural process led to an almost complete freedom of materials and process. A wide variety of materials may be worked by removal such as carving, assembled by welding or modelling, or molded, or cast. (Wikipedia)."@en .


###  http://www.sirma.com/ontologies/2016/02/culturalHeritageConservation/SMK#WorksOfArtOnPaperInMultipleParts
smk:WorksOfArtOnPaperInMultipleParts rdf:type owl:Class ;
                                     rdfs:subClassOf chc:CulturalObject ;
                                     emf:classCategory "culturalobject" ;
                                     emf:definitionId "objectinstance" ;
                                     emf:isCreateable "true"^^xsd:boolean ;
                                     emf:isPartOfObjectLibrary "true"^^xsd:boolean ;
                                     emf:isSearchable "true"^^xsd:boolean ;
                                     dc:creator "Malvina Makrieva"@en ;
                                     sec:allowInheritLibraryPermissions "true"^^xsd:boolean ;
                                     sec:allowInheritParentPermissions "false"^^xsd:boolean ;
                                     rdfs:label "KKS værk i flere dele"@da ,
                                                "Works of Art on Paper in Multiple Parts"@en ;
                                     skos:definition "A work of art on paper in multiple parts is a work of art consisting of several prints, drawings, or photographs which in concept is a single work of art (analogue to installations). The term may also be applied to portfolios or bound volumes such as sketchbooks, artist's books, and printed books etc."@en .


#################################################################
#    Annotations
#################################################################

emf:hasAssignee sec:autoAssignParentPermissionRole "COLLABORATOR" ;
                sec:autoAssignPermissionRole "COLLABORATOR" .


emf:hasPrimaryImage emf:isSearchable "true"^^xsd:boolean .


emf:hasWatcher sec:autoAssignPermissionRole "CONSUMER" .


emf:isPrimaryImageOf emf:isSearchable "true"^^xsd:boolean .


emf:processedBy emf:isSearchable "true"^^xsd:boolean .


emf:processes emf:isSearchable "true"^^xsd:boolean .


ptop:hasParticipant sec:autoAssignPermissionRole "COLLABORATOR" ;
                    sec:autoAssignParentPermissionRole "COLLABORATOR" ;
                    emf:isSearchable "true"^^xsd:boolean ;
                    emf:auditEvent "+addHasParticipant|-removeHasParticipant|changeHasParticipant" .


ptop:involvedIn emf:auditEvent "+addInvolvedIn|-removeInvolvedIn|changeInvolvedIn" ;
                emf:isSearchable "true"^^xsd:boolean .


chc:Exhibition emf:isPartOfObjectLibrary "true"^^xsd:boolean ;
               sec:allowInheritLibraryPermissions "true"^^xsd:boolean ;
               sec:allowInheritParentPermissions "false"^^xsd:boolean ;
               emf:isCreateable "true"^^xsd:boolean ;
               emf:isSearchable "true"^^xsd:boolean .


chc:Sample emf:isCreateable "true"^^xsd:boolean ;
           emf:isPartOfObjectLibrary "true"^^xsd:boolean ;
           emf:isSearchable "true"^^xsd:boolean ;
           sec:allowInheritLibraryPermissions "true"^^xsd:boolean ;
           sec:allowInheritParentPermissions "false"^^xsd:boolean .


chc:approvedBy sec:autoAssignPermissionRole "COLLABORATOR" ;
               sec:autoAssignParentPermissionRole "CONSUMER" ;
               emf:isSearchable "true"^^xsd:boolean .


chc:attachmentOf emf:isSearchable "true"^^xsd:boolean .


chc:documents emf:isSearchable "true"^^xsd:boolean .


chc:duplicates emf:isSearchable "true"^^xsd:boolean .


chc:hasApproved emf:isSearchable "true"^^xsd:boolean .


chc:hasAssignedConservator emf:isSearchable "true"^^xsd:boolean ;
                           sec:autoAssignPermissionRole "COLLABORATOR" ;
                           sec:autoAssignParentPermissionRole "COLLABORATOR" .


chc:hasAttachment emf:isSearchable "true"^^xsd:boolean .


chc:hasSample emf:isSearchable "true"^^xsd:boolean .


chc:isAssignedConservator emf:isSearchable "true"^^xsd:boolean .


chc:isDocumentedIn emf:isSearchable "true"^^xsd:boolean .


chc:isTakenFrom emf:isSearchable "true"^^xsd:boolean .


###  Generated by the OWL API (version 4.2.8.20170104-2310) https://github.com/owlcs/owlapi
